complete coq implementation of task5, bouncing ball

formal/coqimp/debug_printers.mli
@@ -1,0 +1,15 @@
+open BinNums
+open Datatypes
+open Floats
+open Float_text_io
+
+module DebugIO :
+ sig
+  val width : nat
+
+  val fdigs : nat
+
+  val print_float : float -> char list
+
+  val print_Z : coq_Z -> nat -> char list
+ end
