formal/coqimp/digsim_driver.ml
@@ -1,0 +1,94 @@
+open Top
+open Format
+open Debug_printers
+open DebugIO
+open Maps
+open List
+
+let cl2s cl = String.init (List.length cl) (fun i -> (List.nth cl i));;
+let f2s fval = cl2s (print_float fval);;
+let print_sv sv = cl2s (svToStr sv);;
+
+let print_svtree tree =
+  printf "@[SvFloatTree@,";
+  let kvpairs = PTree.elements tree in
+   ignore (map (fun (pos, fval) ->
+      let sv = posToStateVar' pos in
+      let svstring = print_sv sv in
+      let fstr = f2s fval in
+      printf "@[<h>(%s ->@ %s)@ @]" svstring fstr)
+    kvpairs);
+  printf "@]";;
+
+let print_vars sim =
+  printf "@[{vars@,"; print_svtree sim.vars; printf "},@]";;
+
+let print_solkeys sim =
+  printf "@[{solkeys@,";
+  ignore (map (fun sv -> print_string (print_sv sv)) sim.solkeys);
+  printf "},@]";;
+
+let print_row row =
+  printf "@[";
+  ignore (map (fun v -> printf "%s\t" (cl2s v)) row);
+  printf "@]@,";;
+
+let print_solution sim =
+  printf "@[<v 2>{solution@,";
+  ignore (map (fun row -> print_row row) sim.solution);
+  printf "},@]@,";;
+
+let print_event ev =
+  printf "@[{Event@,";
+  printf "@[key=%s,@ time=%s@]@," (cl2s ev.key) (f2s ev.time);
+  printf "}@]@,";;
+
+let print_events sim =
+  printf "@[<v 2>{events@,";
+  ignore (map (fun ev -> print_event ev) sim.sim_events);
+  printf "},@]@,";;
+
+let print_vars sim =
+  printf "@[<hov 2>{vars@,"; print_svtree sim.vars; printf "}@],@]";;
+
+let print_log_entry le =
+  printf "@[<v 2>{log_entry@,";
+  printf "@[caption=%s,@]@ " (cl2s le.le_caption);
+  printf "@[{le_vars=";
+  ignore (map (fun (sv,fval) -> printf "@[%s -> %s@]@ " (cl2s sv) (cl2s fval)) le.le_vars);
+  printf "}@]";
+  printf "@[{le_events=";
+  ignore (map (fun (val1,val2) -> printf "@[%s @ %s@]@ " (cl2s val1) (cl2s val2)) le.le_events);
+  printf "}@]";
+  printf "},@]@,";;
+
+let print_log sim =
+  printf "@[<v 2>{Log@,";
+  ignore (map (fun log_entry -> print_log_entry log_entry) sim.log);
+  printf "}@]@,";;
+
+let print_flags sim =
+  let fl = sim.flags in
+  printf "@[<h>{flags: stop_simulation=%B, end_of_run=%B, evaluate_xd=%B}@]"
+    fl.stop_simulation fl.end_of_run fl.evaluate_xd;;
+
+let print_sim sim =
+  printf "@[<v 2>{simTY@\n";
+  print_vars sim;
+  print_solkeys sim;
+  print_solution sim;
+  print_events sim;
+  print_log sim;
+  print_flags sim;
+  printf "@]}";;
+
+let test =
+  print_newline();
+  let sim = main () in
+  print_sim sim;
+  print_newline();
+  print_endline "This is a test";;
+
+test;;
+
+  
