formal/coqimp/extraction/Top.ml
@@ -1,0 +1,3356 @@
+
+type __ = Obj.t
+let __ = let rec f _ = Obj.repr f in Obj.repr f
+
+(** val xorb : bool -> bool -> bool **)
+
+let xorb b1 b2 =
+  if b1 then if b2 then false else true else b2
+
+(** val negb : bool -> bool **)
+
+let negb = function
+| true -> false
+| false -> true
+
+type nat =
+| O
+| S of nat
+
+(** val app : 'a1 list -> 'a1 list -> 'a1 list **)
+
+let rec app l m =
+  match l with
+  | [] -> m
+  | a :: l1 -> a :: (app l1 m)
+
+type comparison =
+| Eq
+| Lt
+| Gt
+
+(** val compOpp : comparison -> comparison **)
+
+let compOpp = function
+| Eq -> Eq
+| Lt -> Gt
+| Gt -> Lt
+
+type 'a sig0 = 'a
+  (* singleton inductive, whose constructor was exist *)
+
+
+
+type uint =
+| Nil
+| D0 of uint
+| D1 of uint
+| D2 of uint
+| D3 of uint
+| D4 of uint
+| D5 of uint
+| D6 of uint
+| D7 of uint
+| D8 of uint
+| D9 of uint
+
+type int =
+| Pos of uint
+| Neg of uint
+
+(** val nzhead : uint -> uint **)
+
+let rec nzhead d = match d with
+| D0 d0 -> nzhead d0
+| _ -> d
+
+(** val unorm : uint -> uint **)
+
+let unorm d =
+  match nzhead d with
+  | Nil -> D0 Nil
+  | x -> x
+
+(** val norm : int -> int **)
+
+let norm = function
+| Pos d0 -> Pos (unorm d0)
+| Neg d0 -> (match nzhead d0 with
+             | Nil -> Pos (D0 Nil)
+             | x -> Neg x)
+
+(** val pred : nat -> nat **)
+
+let pred n0 = match n0 with
+| O -> n0
+| S u -> u
+
+(** val sub : nat -> nat -> nat **)
+
+let rec sub n0 m =
+  match n0 with
+  | O -> n0
+  | S k -> (match m with
+            | O -> n0
+            | S l -> sub k l)
+
+type ('e, 't) reader = 'e -> 't
+
+(** val constructor : 'a2 -> ('a1, 'a2) reader **)
+
+let constructor x _ =
+  x
+
+type ('r, 't) setter = ('t -> 't) -> 'r -> 'r
+  (* singleton inductive, whose constructor was Build_Setter *)
+
+(** val set : ('a1 -> 'a2) -> ('a1, 'a2) setter -> ('a2 -> 'a2) -> 'a1 -> 'a1 **)
+
+let set _ setter0 =
+  setter0
+
+(** val eqb : bool -> bool -> bool **)
+
+let eqb b1 b2 =
+  if b1 then b2 else if b2 then false else true
+
+module Nat =
+ struct
+  (** val leb : nat -> nat -> bool **)
+
+  let rec leb n0 m =
+    match n0 with
+    | O -> true
+    | S n' -> (match m with
+               | O -> false
+               | S m' -> leb n' m')
+
+  (** val ltb : nat -> nat -> bool **)
+
+  let ltb n0 m =
+    leb (S n0) m
+ end
+
+type positive =
+| XI of positive
+| XO of positive
+| XH
+
+type n =
+| N0
+| Npos of positive
+
+type z =
+| Z0
+| Zpos of positive
+| Zneg of positive
+
+module Pos =
+ struct
+  type mask =
+  | IsNul
+  | IsPos of positive
+  | IsNeg
+ end
+
+module Coq_Pos =
+ struct
+  (** val succ : positive -> positive **)
+
+  let rec succ = function
+  | XI p -> XO (succ p)
+  | XO p -> XI p
+  | XH -> XO XH
+
+  (** val add : positive -> positive -> positive **)
+
+  let rec add x y =
+    match x with
+    | XI p -> (match y with
+               | XI q -> XO (add_carry p q)
+               | XO q -> XI (add p q)
+               | XH -> XO (succ p))
+    | XO p -> (match y with
+               | XI q -> XI (add p q)
+               | XO q -> XO (add p q)
+               | XH -> XI p)
+    | XH -> (match y with
+             | XI q -> XO (succ q)
+             | XO q -> XI q
+             | XH -> XO XH)
+
+  (** val add_carry : positive -> positive -> positive **)
+
+  and add_carry x y =
+    match x with
+    | XI p -> (match y with
+               | XI q -> XI (add_carry p q)
+               | XO q -> XO (add_carry p q)
+               | XH -> XI (succ p))
+    | XO p -> (match y with
+               | XI q -> XO (add_carry p q)
+               | XO q -> XI (add p q)
+               | XH -> XO (succ p))
+    | XH -> (match y with
+             | XI q -> XI (succ q)
+             | XO q -> XO (succ q)
+             | XH -> XI XH)
+
+  (** val pred_double : positive -> positive **)
+
+  let rec pred_double = function
+  | XI p -> XI (XO p)
+  | XO p -> XI (pred_double p)
+  | XH -> XH
+
+  type mask = Pos.mask =
+  | IsNul
+  | IsPos of positive
+  | IsNeg
+
+  (** val succ_double_mask : mask -> mask **)
+
+  let succ_double_mask = function
+  | IsNul -> IsPos XH
+  | IsPos p -> IsPos (XI p)
+  | IsNeg -> IsNeg
+
+  (** val double_mask : mask -> mask **)
+
+  let double_mask = function
+  | IsPos p -> IsPos (XO p)
+  | x0 -> x0
+
+  (** val double_pred_mask : positive -> mask **)
+
+  let double_pred_mask = function
+  | XI p -> IsPos (XO (XO p))
+  | XO p -> IsPos (XO (pred_double p))
+  | XH -> IsNul
+
+  (** val sub_mask : positive -> positive -> mask **)
+
+  let rec sub_mask x y =
+    match x with
+    | XI p ->
+      (match y with
+       | XI q -> double_mask (sub_mask p q)
+       | XO q -> succ_double_mask (sub_mask p q)
+       | XH -> IsPos (XO p))
+    | XO p ->
+      (match y with
+       | XI q -> succ_double_mask (sub_mask_carry p q)
+       | XO q -> double_mask (sub_mask p q)
+       | XH -> IsPos (pred_double p))
+    | XH -> (match y with
+             | XH -> IsNul
+             | _ -> IsNeg)
+
+  (** val sub_mask_carry : positive -> positive -> mask **)
+
+  and sub_mask_carry x y =
+    match x with
+    | XI p ->
+      (match y with
+       | XI q -> succ_double_mask (sub_mask_carry p q)
+       | XO q -> double_mask (sub_mask p q)
+       | XH -> IsPos (pred_double p))
+    | XO p ->
+      (match y with
+       | XI q -> double_mask (sub_mask_carry p q)
+       | XO q -> succ_double_mask (sub_mask_carry p q)
+       | XH -> double_pred_mask p)
+    | XH -> IsNeg
+
+  (** val mul : positive -> positive -> positive **)
+
+  let rec mul x y =
+    match x with
+    | XI p -> add y (XO (mul p y))
+    | XO p -> XO (mul p y)
+    | XH -> y
+
+  (** val iter : ('a1 -> 'a1) -> 'a1 -> positive -> 'a1 **)
+
+  let rec iter f x = function
+  | XI n' -> f (iter f (iter f x n') n')
+  | XO n' -> iter f (iter f x n') n'
+  | XH -> f x
+
+  (** val square : positive -> positive **)
+
+  let rec square = function
+  | XI p0 -> XI (XO (add (square p0) p0))
+  | XO p0 -> XO (XO (square p0))
+  | XH -> XH
+
+  (** val div2 : positive -> positive **)
+
+  let div2 = function
+  | XI p0 -> p0
+  | XO p0 -> p0
+  | XH -> XH
+
+  (** val div2_up : positive -> positive **)
+
+  let div2_up = function
+  | XI p0 -> succ p0
+  | XO p0 -> p0
+  | XH -> XH
+
+  (** val size : positive -> positive **)
+
+  let rec size = function
+  | XI p0 -> succ (size p0)
+  | XO p0 -> succ (size p0)
+  | XH -> XH
+
+  (** val compare_cont : comparison -> positive -> positive -> comparison **)
+
+  let rec compare_cont r x y =
+    match x with
+    | XI p -> (match y with
+               | XI q -> compare_cont r p q
+               | XO q -> compare_cont Gt p q
+               | XH -> Gt)
+    | XO p -> (match y with
+               | XI q -> compare_cont Lt p q
+               | XO q -> compare_cont r p q
+               | XH -> Gt)
+    | XH -> (match y with
+             | XH -> r
+             | _ -> Lt)
+
+  (** val compare : positive -> positive -> comparison **)
+
+  let compare =
+    compare_cont Eq
+
+  (** val eqb : positive -> positive -> bool **)
+
+  let rec eqb p q =
+    match p with
+    | XI p0 -> (match q with
+                | XI q0 -> eqb p0 q0
+                | _ -> false)
+    | XO p0 -> (match q with
+                | XO q0 -> eqb p0 q0
+                | _ -> false)
+    | XH -> (match q with
+             | XH -> true
+             | _ -> false)
+
+  (** val leb : positive -> positive -> bool **)
+
+  let leb x y =
+    match compare x y with
+    | Gt -> false
+    | _ -> true
+
+  (** val sqrtrem_step :
+      (positive -> positive) -> (positive -> positive) -> (positive * mask) -> positive * mask **)
+
+  let sqrtrem_step f g = function
+  | (s, y) ->
+    (match y with
+     | IsPos r ->
+       let s' = XI (XO s) in
+       let r' = g (f r) in if leb s' r' then ((XI s), (sub_mask r' s')) else ((XO s), (IsPos r'))
+     | _ -> ((XO s), (sub_mask (g (f XH)) (XO (XO XH)))))
+
+  (** val sqrtrem : positive -> positive * mask **)
+
+  let rec sqrtrem = function
+  | XI p0 ->
+    (match p0 with
+     | XI p1 -> sqrtrem_step (fun x -> XI x) (fun x -> XI x) (sqrtrem p1)
+     | XO p1 -> sqrtrem_step (fun x -> XO x) (fun x -> XI x) (sqrtrem p1)
+     | XH -> (XH, (IsPos (XO XH))))
+  | XO p0 ->
+    (match p0 with
+     | XI p1 -> sqrtrem_step (fun x -> XI x) (fun x -> XO x) (sqrtrem p1)
+     | XO p1 -> sqrtrem_step (fun x -> XO x) (fun x -> XO x) (sqrtrem p1)
+     | XH -> (XH, (IsPos XH)))
+  | XH -> (XH, IsNul)
+
+  (** val coq_lor : positive -> positive -> positive **)
+
+  let rec coq_lor p q =
+    match p with
+    | XI p0 -> (match q with
+                | XI q0 -> XI (coq_lor p0 q0)
+                | XO q0 -> XI (coq_lor p0 q0)
+                | XH -> p)
+    | XO p0 -> (match q with
+                | XI q0 -> XI (coq_lor p0 q0)
+                | XO q0 -> XO (coq_lor p0 q0)
+                | XH -> XI p0)
+    | XH -> (match q with
+             | XO q0 -> XI q0
+             | _ -> q)
+
+  (** val of_succ_nat : nat -> positive **)
+
+  let rec of_succ_nat = function
+  | O -> XH
+  | S x -> succ (of_succ_nat x)
+
+  (** val of_uint_acc : uint -> positive -> positive **)
+
+  let rec of_uint_acc d acc =
+    match d with
+    | Nil -> acc
+    | D0 l -> of_uint_acc l (mul (XO (XI (XO XH))) acc)
+    | D1 l -> of_uint_acc l (add XH (mul (XO (XI (XO XH))) acc))
+    | D2 l -> of_uint_acc l (add (XO XH) (mul (XO (XI (XO XH))) acc))
+    | D3 l -> of_uint_acc l (add (XI XH) (mul (XO (XI (XO XH))) acc))
+    | D4 l -> of_uint_acc l (add (XO (XO XH)) (mul (XO (XI (XO XH))) acc))
+    | D5 l -> of_uint_acc l (add (XI (XO XH)) (mul (XO (XI (XO XH))) acc))
+    | D6 l -> of_uint_acc l (add (XO (XI XH)) (mul (XO (XI (XO XH))) acc))
+    | D7 l -> of_uint_acc l (add (XI (XI XH)) (mul (XO (XI (XO XH))) acc))
+    | D8 l -> of_uint_acc l (add (XO (XO (XO XH))) (mul (XO (XI (XO XH))) acc))
+    | D9 l -> of_uint_acc l (add (XI (XO (XO XH))) (mul (XO (XI (XO XH))) acc))
+
+  (** val of_uint : uint -> n **)
+
+  let rec of_uint = function
+  | Nil -> N0
+  | D0 l -> of_uint l
+  | D1 l -> Npos (of_uint_acc l XH)
+  | D2 l -> Npos (of_uint_acc l (XO XH))
+  | D3 l -> Npos (of_uint_acc l (XI XH))
+  | D4 l -> Npos (of_uint_acc l (XO (XO XH)))
+  | D5 l -> Npos (of_uint_acc l (XI (XO XH)))
+  | D6 l -> Npos (of_uint_acc l (XO (XI XH)))
+  | D7 l -> Npos (of_uint_acc l (XI (XI XH)))
+  | D8 l -> Npos (of_uint_acc l (XO (XO (XO XH))))
+  | D9 l -> Npos (of_uint_acc l (XI (XO (XO XH))))
+
+  (** val eq_dec : positive -> positive -> bool **)
+
+  let rec eq_dec p x0 =
+    match p with
+    | XI p0 -> (match x0 with
+                | XI p1 -> eq_dec p0 p1
+                | _ -> false)
+    | XO p0 -> (match x0 with
+                | XO p1 -> eq_dec p0 p1
+                | _ -> false)
+    | XH -> (match x0 with
+             | XH -> true
+             | _ -> false)
+ end
+
+(** val rev : 'a1 list -> 'a1 list **)
+
+let rec rev = function
+| [] -> []
+| x :: l' -> app (rev l') (x :: [])
+
+module Z =
+ struct
+  (** val double : z -> z **)
+
+  let double = function
+  | Z0 -> Z0
+  | Zpos p -> Zpos (XO p)
+  | Zneg p -> Zneg (XO p)
+
+  (** val succ_double : z -> z **)
+
+  let succ_double = function
+  | Z0 -> Zpos XH
+  | Zpos p -> Zpos (XI p)
+  | Zneg p -> Zneg (Coq_Pos.pred_double p)
+
+  (** val pred_double : z -> z **)
+
+  let pred_double = function
+  | Z0 -> Zneg XH
+  | Zpos p -> Zpos (Coq_Pos.pred_double p)
+  | Zneg p -> Zneg (XI p)
+
+  (** val pos_sub : positive -> positive -> z **)
+
+  let rec pos_sub x y =
+    match x with
+    | XI p ->
+      (match y with
+       | XI q -> double (pos_sub p q)
+       | XO q -> succ_double (pos_sub p q)
+       | XH -> Zpos (XO p))
+    | XO p ->
+      (match y with
+       | XI q -> pred_double (pos_sub p q)
+       | XO q -> double (pos_sub p q)
+       | XH -> Zpos (Coq_Pos.pred_double p))
+    | XH -> (match y with
+             | XI q -> Zneg (XO q)
+             | XO q -> Zneg (Coq_Pos.pred_double q)
+             | XH -> Z0)
+
+  (** val add : z -> z -> z **)
+
+  let add x y =
+    match x with
+    | Z0 -> y
+    | Zpos x' -> (match y with
+                  | Z0 -> x
+                  | Zpos y' -> Zpos (Coq_Pos.add x' y')
+                  | Zneg y' -> pos_sub x' y')
+    | Zneg x' -> (match y with
+                  | Z0 -> x
+                  | Zpos y' -> pos_sub y' x'
+                  | Zneg y' -> Zneg (Coq_Pos.add x' y'))
+
+  (** val opp : z -> z **)
+
+  let opp = function
+  | Z0 -> Z0
+  | Zpos x0 -> Zneg x0
+  | Zneg x0 -> Zpos x0
+
+  (** val succ : z -> z **)
+
+  let succ x =
+    add x (Zpos XH)
+
+  (** val pred : z -> z **)
+
+  let pred x =
+    add x (Zneg XH)
+
+  (** val sub : z -> z -> z **)
+
+  let sub m n0 =
+    add m (opp n0)
+
+  (** val mul : z -> z -> z **)
+
+  let mul x y =
+    match x with
+    | Z0 -> Z0
+    | Zpos x' ->
+      (match y with
+       | Z0 -> Z0
+       | Zpos y' -> Zpos (Coq_Pos.mul x' y')
+       | Zneg y' -> Zneg (Coq_Pos.mul x' y'))
+    | Zneg x' ->
+      (match y with
+       | Z0 -> Z0
+       | Zpos y' -> Zneg (Coq_Pos.mul x' y')
+       | Zneg y' -> Zpos (Coq_Pos.mul x' y'))
+
+  (** val pow_pos : z -> positive -> z **)
+
+  let pow_pos z0 =
+    Coq_Pos.iter (mul z0) (Zpos XH)
+
+  (** val pow : z -> z -> z **)
+
+  let pow x = function
+  | Z0 -> Zpos XH
+  | Zpos p -> pow_pos x p
+  | Zneg _ -> Z0
+
+  (** val compare : z -> z -> comparison **)
+
+  let compare x y =
+    match x with
+    | Z0 -> (match y with
+             | Z0 -> Eq
+             | Zpos _ -> Lt
+             | Zneg _ -> Gt)
+    | Zpos x' -> (match y with
+                  | Zpos y' -> Coq_Pos.compare x' y'
+                  | _ -> Gt)
+    | Zneg x' -> (match y with
+                  | Zneg y' -> compOpp (Coq_Pos.compare x' y')
+                  | _ -> Lt)
+
+  (** val leb : z -> z -> bool **)
+
+  let leb x y =
+    match compare x y with
+    | Gt -> false
+    | _ -> true
+
+  (** val ltb : z -> z -> bool **)
+
+  let ltb x y =
+    match compare x y with
+    | Lt -> true
+    | _ -> false
+
+  (** val eqb : z -> z -> bool **)
+
+  let rec eqb x y =
+    match x with
+    | Z0 -> (match y with
+             | Z0 -> true
+             | _ -> false)
+    | Zpos p -> (match y with
+                 | Zpos q -> Coq_Pos.eqb p q
+                 | _ -> false)
+    | Zneg p -> (match y with
+                 | Zneg q -> Coq_Pos.eqb p q
+                 | _ -> false)
+
+  (** val max : z -> z -> z **)
+
+  let max n0 m =
+    match compare n0 m with
+    | Lt -> m
+    | _ -> n0
+
+  (** val min : z -> z -> z **)
+
+  let min n0 m =
+    match compare n0 m with
+    | Gt -> m
+    | _ -> n0
+
+  (** val of_nat : nat -> z **)
+
+  let of_nat = function
+  | O -> Z0
+  | S n1 -> Zpos (Coq_Pos.of_succ_nat n1)
+
+  (** val of_N : n -> z **)
+
+  let of_N = function
+  | N0 -> Z0
+  | Npos p -> Zpos p
+
+  (** val of_uint : uint -> z **)
+
+  let of_uint d =
+    of_N (Coq_Pos.of_uint d)
+
+  (** val of_int : int -> z **)
+
+  let of_int = function
+  | Pos d0 -> of_uint d0
+  | Neg d0 -> opp (of_uint d0)
+
+  (** val pos_div_eucl : positive -> z -> z * z **)
+
+  let rec pos_div_eucl a b =
+    match a with
+    | XI a' ->
+      let (q, r) = pos_div_eucl a' b in
+      let r' = add (mul (Zpos (XO XH)) r) (Zpos XH) in
+      if ltb r' b then ((mul (Zpos (XO XH)) q), r') else ((add (mul (Zpos (XO XH)) q) (Zpos XH)), (sub r' b))
+    | XO a' ->
+      let (q, r) = pos_div_eucl a' b in
+      let r' = mul (Zpos (XO XH)) r in
+      if ltb r' b then ((mul (Zpos (XO XH)) q), r') else ((add (mul (Zpos (XO XH)) q) (Zpos XH)), (sub r' b))
+    | XH -> if leb (Zpos (XO XH)) b then (Z0, (Zpos XH)) else ((Zpos XH), Z0)
+
+  (** val div_eucl : z -> z -> z * z **)
+
+  let div_eucl a b =
+    match a with
+    | Z0 -> (Z0, Z0)
+    | Zpos a' ->
+      (match b with
+       | Z0 -> (Z0, Z0)
+       | Zpos _ -> pos_div_eucl a' b
+       | Zneg b' ->
+         let (q, r) = pos_div_eucl a' (Zpos b') in
+         (match r with
+          | Z0 -> ((opp q), Z0)
+          | _ -> ((opp (add q (Zpos XH))), (add b r))))
+    | Zneg a' ->
+      (match b with
+       | Z0 -> (Z0, Z0)
+       | Zpos _ ->
+         let (q, r) = pos_div_eucl a' b in
+         (match r with
+          | Z0 -> ((opp q), Z0)
+          | _ -> ((opp (add q (Zpos XH))), (sub b r)))
+       | Zneg b' -> let (q, r) = pos_div_eucl a' (Zpos b') in (q, (opp r)))
+
+  (** val div : z -> z -> z **)
+
+  let div a b =
+    let (q, _) = div_eucl a b in q
+
+  (** val modulo : z -> z -> z **)
+
+  let modulo a b =
+    let (_, r) = div_eucl a b in r
+
+  (** val div2 : z -> z **)
+
+  let div2 = function
+  | Z0 -> Z0
+  | Zpos p -> (match p with
+               | XH -> Z0
+               | _ -> Zpos (Coq_Pos.div2 p))
+  | Zneg p -> Zneg (Coq_Pos.div2_up p)
+
+  (** val log2 : z -> z **)
+
+  let log2 = function
+  | Zpos p0 -> (match p0 with
+                | XI p -> Zpos (Coq_Pos.size p)
+                | XO p -> Zpos (Coq_Pos.size p)
+                | XH -> Z0)
+  | _ -> Z0
+
+  (** val sqrtrem : z -> z * z **)
+
+  let sqrtrem = function
+  | Zpos p ->
+    let (s, m) = Coq_Pos.sqrtrem p in
+    (match m with
+     | Coq_Pos.IsPos r -> ((Zpos s), (Zpos r))
+     | _ -> ((Zpos s), Z0))
+  | _ -> (Z0, Z0)
+
+  (** val shiftl : z -> z -> z **)
+
+  let shiftl a = function
+  | Z0 -> a
+  | Zpos p -> Coq_Pos.iter (mul (Zpos (XO XH))) a p
+  | Zneg p -> Coq_Pos.iter div2 a p
+
+  (** val eq_dec : z -> z -> bool **)
+
+  let eq_dec x y =
+    match x with
+    | Z0 -> (match y with
+             | Z0 -> true
+             | _ -> false)
+    | Zpos x0 -> (match y with
+                  | Zpos p0 -> Coq_Pos.eq_dec x0 p0
+                  | _ -> false)
+    | Zneg x0 -> (match y with
+                  | Zneg p0 -> Coq_Pos.eq_dec x0 p0
+                  | _ -> false)
+
+  (** val log2_up : z -> z **)
+
+  let log2_up a =
+    match compare (Zpos XH) a with
+    | Lt -> succ (log2 (pred a))
+    | _ -> Z0
+ end
+
+(** val z_lt_dec : z -> z -> bool **)
+
+let z_lt_dec x y =
+  match Z.compare x y with
+  | Lt -> true
+  | _ -> false
+
+(** val z_le_dec : z -> z -> bool **)
+
+let z_le_dec x y =
+  match Z.compare x y with
+  | Gt -> false
+  | _ -> true
+
+(** val z_le_gt_dec : z -> z -> bool **)
+
+let z_le_gt_dec =
+  z_le_dec
+
+(** val zeq_bool : z -> z -> bool **)
+
+let zeq_bool x y =
+  match Z.compare x y with
+  | Eq -> true
+  | _ -> false
+
+(** val append : char list -> char list -> char list **)
+
+let rec append s1 s2 =
+  match s1 with
+  | [] -> s2
+  | c::s1' -> c::(append s1' s2)
+
+(** val length : char list -> nat **)
+
+let rec length = function
+| [] -> O
+| _::s' -> S (length s')
+
+(** val substring : nat -> nat -> char list -> char list **)
+
+let rec substring n0 m s =
+  match n0 with
+  | O -> (match m with
+          | O -> []
+          | S m' -> (match s with
+                     | [] -> s
+                     | c::s' -> c::(substring O m' s')))
+  | S n' -> (match s with
+             | [] -> s
+             | _::s' -> substring n' m s')
+
+(** val prefix : char list -> char list -> bool **)
+
+let rec prefix s1 s2 =
+  match s1 with
+  | [] -> true
+  | a::s1' -> (match s2 with
+               | [] -> false
+               | b::s2' -> if (=) a b then prefix s1' s2' else false)
+
+(** val index : nat -> char list -> char list -> nat option **)
+
+let rec index n0 s1 s2 = match s2 with
+| [] -> (match n0 with
+         | O -> (match s1 with
+                 | [] -> Some O
+                 | _::_ -> None)
+         | S _ -> None)
+| _::s2' ->
+  (match n0 with
+   | O -> if prefix s1 s2 then Some O else (match index O s1 s2' with
+                                            | Some n1 -> Some (S n1)
+                                            | None -> None)
+   | S n' -> (match index n' s1 s2' with
+              | Some n1 -> Some (S n1)
+              | None -> None))
+
+(** val shift_nat : nat -> positive -> positive **)
+
+let rec shift_nat n0 z0 =
+  match n0 with
+  | O -> z0
+  | S n1 -> XO (shift_nat n1 z0)
+
+(** val shift_pos : positive -> positive -> positive **)
+
+let shift_pos n0 z0 =
+  Coq_Pos.iter (fun x -> XO x) z0 n0
+
+(** val two_power_nat : nat -> z **)
+
+let two_power_nat n0 =
+  Zpos (shift_nat n0 XH)
+
+(** val zeq : z -> z -> bool **)
+
+let zeq =
+  Z.eq_dec
+
+(** val zlt : z -> z -> bool **)
+
+let zlt =
+  z_lt_dec
+
+(** val zle : z -> z -> bool **)
+
+let zle =
+  z_le_gt_dec
+
+(** val option_map : ('a1 -> 'a2) -> 'a1 option -> 'a2 option **)
+
+let option_map f = function
+| Some y -> Some (f y)
+| None -> None
+
+(** val zeven : z -> bool **)
+
+let zeven = function
+| Z0 -> true
+| Zpos p -> (match p with
+             | XO _ -> true
+             | _ -> false)
+| Zneg p -> (match p with
+             | XO _ -> true
+             | _ -> false)
+
+type radix = z
+  (* singleton inductive, whose constructor was Build_radix *)
+
+(** val radix_val : radix -> z **)
+
+let radix_val r =
+  r
+
+(** val radix2 : radix **)
+
+let radix2 =
+  Zpos (XO XH)
+
+(** val cond_Zopp : bool -> z -> z **)
+
+let cond_Zopp b m =
+  if b then Z.opp m else m
+
+(** val zpos_div_eucl_aux1 : positive -> positive -> z * z **)
+
+let rec zpos_div_eucl_aux1 a b = match b with
+| XI _ -> Z.pos_div_eucl a (Zpos b)
+| XO b' ->
+  (match a with
+   | XI a' -> let (q, r) = zpos_div_eucl_aux1 a' b' in (q, (Z.add (Z.mul (Zpos (XO XH)) r) (Zpos XH)))
+   | XO a' -> let (q, r) = zpos_div_eucl_aux1 a' b' in (q, (Z.mul (Zpos (XO XH)) r))
+   | XH -> (Z0, (Zpos a)))
+| XH -> ((Zpos a), Z0)
+
+(** val zpos_div_eucl_aux : positive -> positive -> z * z **)
+
+let zpos_div_eucl_aux a b =
+  match Coq_Pos.compare a b with
+  | Eq -> ((Zpos XH), Z0)
+  | Lt -> (Z0, (Zpos a))
+  | Gt -> zpos_div_eucl_aux1 a b
+
+(** val zfast_div_eucl : z -> z -> z * z **)
+
+let zfast_div_eucl a b =
+  match a with
+  | Z0 -> (Z0, Z0)
+  | Zpos a' ->
+    (match b with
+     | Z0 -> (Z0, Z0)
+     | Zpos b' -> zpos_div_eucl_aux a' b'
+     | Zneg b' ->
+       let (q, r) = zpos_div_eucl_aux a' b' in
+       (match r with
+        | Z0 -> ((Z.opp q), Z0)
+        | _ -> ((Z.opp (Z.add q (Zpos XH))), (Z.add b r))))
+  | Zneg a' ->
+    (match b with
+     | Z0 -> (Z0, Z0)
+     | Zpos b' ->
+       let (q, r) = zpos_div_eucl_aux a' b' in
+       (match r with
+        | Z0 -> ((Z.opp q), Z0)
+        | _ -> ((Z.opp (Z.add q (Zpos XH))), (Z.sub b r)))
+     | Zneg b' -> let (q, r) = zpos_div_eucl_aux a' b' in (q, (Z.opp r)))
+
+(** val iter_nat : ('a1 -> 'a1) -> nat -> 'a1 -> 'a1 **)
+
+let rec iter_nat f n0 x =
+  match n0 with
+  | O -> x
+  | S n' -> iter_nat f n' (f x)
+
+(** val iter_pos : ('a1 -> 'a1) -> positive -> 'a1 -> 'a1 **)
+
+let rec iter_pos f n0 x =
+  match n0 with
+  | XI n' -> iter_pos f n' (iter_pos f n' (f x))
+  | XO n' -> iter_pos f n' (iter_pos f n' x)
+  | XH -> f x
+
+(** val fLT_exp : z -> z -> z -> z **)
+
+let fLT_exp emin prec e =
+  Z.max (Z.sub e prec) emin
+
+(** val digits2_pos : positive -> positive **)
+
+let rec digits2_pos = function
+| XI p -> Coq_Pos.succ (digits2_pos p)
+| XO p -> Coq_Pos.succ (digits2_pos p)
+| XH -> XH
+
+(** val zdigits2 : z -> z **)
+
+let zdigits2 n0 = match n0 with
+| Z0 -> n0
+| Zpos p -> Zpos (digits2_pos p)
+| Zneg p -> Zpos (digits2_pos p)
+
+type location =
+| Loc_Exact
+| Loc_Inexact of comparison
+
+(** val new_location_even : z -> z -> location -> location **)
+
+let new_location_even nb_steps k l =
+  if zeq_bool k Z0
+  then (match l with
+        | Loc_Exact -> l
+        | Loc_Inexact _ -> Loc_Inexact Lt)
+  else Loc_Inexact
+         (match Z.compare (Z.mul (Zpos (XO XH)) k) nb_steps with
+          | Eq -> (match l with
+                   | Loc_Exact -> Eq
+                   | Loc_Inexact _ -> Gt)
+          | x -> x)
+
+(** val new_location_odd : z -> z -> location -> location **)
+
+let new_location_odd nb_steps k l =
+  if zeq_bool k Z0
+  then (match l with
+        | Loc_Exact -> l
+        | Loc_Inexact _ -> Loc_Inexact Lt)
+  else Loc_Inexact
+         (match Z.compare (Z.add (Z.mul (Zpos (XO XH)) k) (Zpos XH)) nb_steps with
+          | Eq -> (match l with
+                   | Loc_Exact -> Lt
+                   | Loc_Inexact l0 -> l0)
+          | x -> x)
+
+(** val new_location : z -> z -> location -> location **)
+
+let new_location nb_steps =
+  if zeven nb_steps then new_location_even nb_steps else new_location_odd nb_steps
+
+(** val cond_incr : bool -> z -> z **)
+
+let cond_incr b m =
+  if b then Z.add m (Zpos XH) else m
+
+(** val round_sign_DN : bool -> location -> bool **)
+
+let round_sign_DN s = function
+| Loc_Exact -> false
+| Loc_Inexact _ -> s
+
+(** val round_sign_UP : bool -> location -> bool **)
+
+let round_sign_UP s = function
+| Loc_Exact -> false
+| Loc_Inexact _ -> negb s
+
+(** val round_N : bool -> location -> bool **)
+
+let round_N p = function
+| Loc_Exact -> false
+| Loc_Inexact c -> (match c with
+                    | Eq -> p
+                    | Lt -> false
+                    | Gt -> true)
+
+type full_float =
+| F754_zero of bool
+| F754_infinity of bool
+| F754_nan of bool * positive
+| F754_finite of bool * positive * z
+
+type nan_pl = positive
+
+type binary_float =
+| B754_zero of bool
+| B754_infinity of bool
+| B754_nan of bool * nan_pl
+| B754_finite of bool * positive * z
+
+(** val fF2B : z -> z -> full_float -> binary_float **)
+
+let fF2B _ _ = function
+| F754_zero s -> B754_zero s
+| F754_infinity s -> B754_infinity s
+| F754_nan (b, pl) -> B754_nan (b, pl)
+| F754_finite (s, m, e) -> B754_finite (s, m, e)
+
+(** val bopp : z -> z -> (bool -> nan_pl -> bool * nan_pl) -> binary_float -> binary_float **)
+
+let bopp _ _ opp_nan = function
+| B754_zero sx -> B754_zero (negb sx)
+| B754_infinity sx -> B754_infinity (negb sx)
+| B754_nan (sx, plx) -> let (sres, plres) = opp_nan sx plx in B754_nan (sres, plres)
+| B754_finite (sx, mx, ex) -> B754_finite ((negb sx), mx, ex)
+
+(** val babs : z -> z -> (bool -> nan_pl -> bool * nan_pl) -> binary_float -> binary_float **)
+
+let babs _ _ abs_nan = function
+| B754_zero _ -> B754_zero false
+| B754_infinity _ -> B754_infinity false
+| B754_nan (sx, plx) -> let (sres, plres) = abs_nan sx plx in B754_nan (sres, plres)
+| B754_finite (_, mx, ex) -> B754_finite (false, mx, ex)
+
+(** val bcompare : z -> z -> binary_float -> binary_float -> comparison option **)
+
+let bcompare _ _ f1 f2 =
+  match f1 with
+  | B754_zero _ ->
+    (match f2 with
+     | B754_zero _ -> Some Eq
+     | B754_infinity b -> if b then Some Gt else Some Lt
+     | B754_nan (_, _) -> None
+     | B754_finite (b, _, _) -> if b then Some Gt else Some Lt)
+  | B754_infinity b ->
+    if b
+    then (match f2 with
+          | B754_infinity b0 -> if b0 then Some Eq else Some Lt
+          | B754_nan (_, _) -> None
+          | _ -> Some Lt)
+    else (match f2 with
+          | B754_infinity b0 -> if b0 then Some Gt else Some Eq
+          | B754_nan (_, _) -> None
+          | _ -> Some Gt)
+  | B754_nan (_, _) -> None
+  | B754_finite (s1, m1, e1) ->
+    if s1
+    then (match f2 with
+          | B754_zero _ -> Some Lt
+          | B754_infinity b -> if b then Some Gt else Some Lt
+          | B754_nan (_, _) -> None
+          | B754_finite (s2, m2, e2) ->
+            if s1
+            then if s2
+                 then (match Z.compare e1 e2 with
+                       | Eq -> Some (compOpp (Coq_Pos.compare_cont Eq m1 m2))
+                       | Lt -> Some Gt
+                       | Gt -> Some Lt)
+                 else Some Lt
+            else if s2
+                 then Some Gt
+                 else (match Z.compare e1 e2 with
+                       | Eq -> Some (Coq_Pos.compare_cont Eq m1 m2)
+                       | x -> Some x))
+    else (match f2 with
+          | B754_zero _ -> Some Gt
+          | B754_infinity b -> if b then Some Gt else Some Lt
+          | B754_nan (_, _) -> None
+          | B754_finite (s2, m2, e2) ->
+            if s1
+            then if s2
+                 then (match Z.compare e1 e2 with
+                       | Eq -> Some (compOpp (Coq_Pos.compare_cont Eq m1 m2))
+                       | Lt -> Some Gt
+                       | Gt -> Some Lt)
+                 else Some Lt
+            else if s2
+                 then Some Gt
+                 else (match Z.compare e1 e2 with
+                       | Eq -> Some (Coq_Pos.compare_cont Eq m1 m2)
+                       | x -> Some x))
+
+type shr_record = { shr_m : z; shr_r : bool; shr_s : bool }
+
+(** val shr_m : shr_record -> z **)
+
+let shr_m x = x.shr_m
+
+(** val shr_1 : shr_record -> shr_record **)
+
+let shr_1 mrs =
+  let { shr_m = m; shr_r = r; shr_s = s } = mrs in
+  let s0 = (||) r s in
+  (match m with
+   | Z0 -> { shr_m = Z0; shr_r = false; shr_s = s0 }
+   | Zpos p0 ->
+     (match p0 with
+      | XI p -> { shr_m = (Zpos p); shr_r = true; shr_s = s0 }
+      | XO p -> { shr_m = (Zpos p); shr_r = false; shr_s = s0 }
+      | XH -> { shr_m = Z0; shr_r = true; shr_s = s0 })
+   | Zneg p0 ->
+     (match p0 with
+      | XI p -> { shr_m = (Zneg p); shr_r = true; shr_s = s0 }
+      | XO p -> { shr_m = (Zneg p); shr_r = false; shr_s = s0 }
+      | XH -> { shr_m = Z0; shr_r = true; shr_s = s0 }))
+
+(** val loc_of_shr_record : shr_record -> location **)
+
+let loc_of_shr_record mrs =
+  let { shr_m = _; shr_r = shr_r0; shr_s = shr_s0 } = mrs in
+  if shr_r0
+  then if shr_s0 then Loc_Inexact Gt else Loc_Inexact Eq
+  else if shr_s0 then Loc_Inexact Lt else Loc_Exact
+
+(** val shr_record_of_loc : z -> location -> shr_record **)
+
+let shr_record_of_loc m = function
+| Loc_Exact -> { shr_m = m; shr_r = false; shr_s = false }
+| Loc_Inexact c ->
+  (match c with
+   | Eq -> { shr_m = m; shr_r = true; shr_s = false }
+   | Lt -> { shr_m = m; shr_r = false; shr_s = true }
+   | Gt -> { shr_m = m; shr_r = true; shr_s = true })
+
+(** val shr : shr_record -> z -> z -> shr_record * z **)
+
+let shr mrs e n0 = match n0 with
+| Zpos p -> ((iter_pos shr_1 p mrs), (Z.add e n0))
+| _ -> (mrs, e)
+
+(** val shr_fexp : z -> z -> z -> z -> location -> shr_record * z **)
+
+let shr_fexp prec emax =
+  let emin = Z.sub (Z.sub (Zpos (XI XH)) emax) prec in
+  let fexp = fLT_exp emin prec in
+  (fun m e l -> shr (shr_record_of_loc m l) e (Z.sub (fexp (Z.add (zdigits2 m) e)) e))
+
+type mode =
+| Mode_NE
+| Mode_ZR
+| Mode_DN
+| Mode_UP
+| Mode_NA
+
+(** val choice_mode : mode -> bool -> z -> location -> z **)
+
+let choice_mode m sx mx lx =
+  match m with
+  | Mode_NE -> cond_incr (round_N (negb (zeven mx)) lx) mx
+  | Mode_ZR -> mx
+  | Mode_DN -> cond_incr (round_sign_DN sx lx) mx
+  | Mode_UP -> cond_incr (round_sign_UP sx lx) mx
+  | Mode_NA -> cond_incr (round_N true lx) mx
+
+(** val overflow_to_inf : mode -> bool -> bool **)
+
+let overflow_to_inf m s =
+  match m with
+  | Mode_ZR -> false
+  | Mode_DN -> s
+  | Mode_UP -> negb s
+  | _ -> true
+
+(** val binary_overflow : z -> z -> mode -> bool -> full_float **)
+
+let binary_overflow prec emax m s =
+  if overflow_to_inf m s
+  then F754_infinity s
+  else F754_finite (s, (match Z.sub (Z.pow (Zpos (XO XH)) prec) (Zpos XH) with
+                        | Zpos p -> p
+                        | _ -> XH), (Z.sub emax prec))
+
+(** val binary_round_aux : z -> z -> mode -> bool -> positive -> z -> location -> full_float **)
+
+let binary_round_aux prec emax mode0 sx mx ex lx =
+  let (mrs', e') = shr_fexp prec emax (Zpos mx) ex lx in
+  let (mrs'', e'') =
+    shr_fexp prec emax (choice_mode mode0 sx mrs'.shr_m (loc_of_shr_record mrs')) e' Loc_Exact
+  in
+  (match mrs''.shr_m with
+   | Z0 -> F754_zero sx
+   | Zpos m ->
+     if Z.leb e'' (Z.sub emax prec) then F754_finite (sx, m, e'') else binary_overflow prec emax mode0 sx
+   | Zneg _ -> F754_nan (false, XH))
+
+(** val bmult :
+    z -> z -> (binary_float -> binary_float -> bool * nan_pl) -> mode -> binary_float -> binary_float ->
+    binary_float **)
+
+let bmult prec emax mult_nan m x y =
+  let f = fun pl -> B754_nan ((fst pl), (snd pl)) in
+  (match x with
+   | B754_zero sx ->
+     (match y with
+      | B754_zero sy -> B754_zero (xorb sx sy)
+      | B754_finite (sy, _, _) -> B754_zero (xorb sx sy)
+      | _ -> f (mult_nan x y))
+   | B754_infinity sx ->
+     (match y with
+      | B754_infinity sy -> B754_infinity (xorb sx sy)
+      | B754_finite (sy, _, _) -> B754_infinity (xorb sx sy)
+      | _ -> f (mult_nan x y))
+   | B754_nan (_, _) -> f (mult_nan x y)
+   | B754_finite (sx, mx, ex) ->
+     (match y with
+      | B754_zero sy -> B754_zero (xorb sx sy)
+      | B754_infinity sy -> B754_infinity (xorb sx sy)
+      | B754_nan (_, _) -> f (mult_nan x y)
+      | B754_finite (sy, my, ey) ->
+        fF2B prec emax (binary_round_aux prec emax m (xorb sx sy) (Coq_Pos.mul mx my) (Z.add ex ey) Loc_Exact)))
+
+(** val shl_align : positive -> z -> z -> positive * z **)
+
+let shl_align mx ex ex' =
+  match Z.sub ex' ex with
+  | Zneg d -> ((shift_pos d mx), ex')
+  | _ -> (mx, ex)
+
+(** val shl_align_fexp : z -> z -> positive -> z -> positive * z **)
+
+let shl_align_fexp prec emax =
+  let emin = Z.sub (Z.sub (Zpos (XI XH)) emax) prec in
+  let fexp = fLT_exp emin prec in (fun mx ex -> shl_align mx ex (fexp (Z.add (Zpos (digits2_pos mx)) ex)))
+
+(** val binary_round : z -> z -> mode -> bool -> positive -> z -> full_float **)
+
+let binary_round prec emax m sx mx ex =
+  let (mz, ez) = shl_align_fexp prec emax mx ex in binary_round_aux prec emax m sx mz ez Loc_Exact
+
+(** val binary_normalize : z -> z -> mode -> z -> z -> bool -> binary_float **)
+
+let binary_normalize prec emax mode0 m e szero =
+  match m with
+  | Z0 -> B754_zero szero
+  | Zpos m0 -> fF2B prec emax (binary_round prec emax mode0 false m0 e)
+  | Zneg m0 -> fF2B prec emax (binary_round prec emax mode0 true m0 e)
+
+(** val bplus :
+    z -> z -> (binary_float -> binary_float -> bool * nan_pl) -> mode -> binary_float -> binary_float ->
+    binary_float **)
+
+let bplus prec emax plus_nan m x y =
+  let f = fun pl -> B754_nan ((fst pl), (snd pl)) in
+  (match x with
+   | B754_zero sx ->
+     (match y with
+      | B754_zero sy ->
+        if eqb sx sy then x else (match m with
+                                  | Mode_DN -> B754_zero true
+                                  | _ -> B754_zero false)
+      | B754_nan (_, _) -> f (plus_nan x y)
+      | _ -> y)
+   | B754_infinity sx ->
+     (match y with
+      | B754_infinity sy -> if eqb sx sy then x else f (plus_nan x y)
+      | B754_nan (_, _) -> f (plus_nan x y)
+      | _ -> x)
+   | B754_nan (_, _) -> f (plus_nan x y)
+   | B754_finite (sx, mx, ex) ->
+     (match y with
+      | B754_zero _ -> x
+      | B754_infinity _ -> y
+      | B754_nan (_, _) -> f (plus_nan x y)
+      | B754_finite (sy, my, ey) ->
+        let ez = Z.min ex ey in
+        binary_normalize prec emax m
+          (Z.add (cond_Zopp sx (Zpos (fst (shl_align mx ex ez))))
+            (cond_Zopp sy (Zpos (fst (shl_align my ey ez))))) ez (match m with
+                                                                  | Mode_DN -> true
+                                                                  | _ -> false)))
+
+(** val bminus :
+    z -> z -> (binary_float -> binary_float -> bool * nan_pl) -> mode -> binary_float -> binary_float ->
+    binary_float **)
+
+let bminus prec emax minus_nan m x y =
+  bplus prec emax minus_nan m x (bopp prec emax (fun x0 x1 -> (x0, x1)) y)
+
+(** val fdiv_core_binary : z -> z -> z -> z -> z -> (z * z) * location **)
+
+let fdiv_core_binary prec m1 e1 m2 e2 =
+  let d1 = zdigits2 m1 in
+  let d2 = zdigits2 m2 in
+  let e = Z.sub e1 e2 in
+  (match Z.sub (Z.add d2 prec) d1 with
+   | Zpos p ->
+     let m = Z.shiftl m1 (Zpos p) in
+     let e' = Z.add e (Zneg p) in let (q, r) = zfast_div_eucl m m2 in ((q, e'), (new_location m2 r Loc_Exact))
+   | _ -> let (q, r) = zfast_div_eucl m1 m2 in ((q, e), (new_location m2 r Loc_Exact)))
+
+(** val bdiv :
+    z -> z -> (binary_float -> binary_float -> bool * nan_pl) -> mode -> binary_float -> binary_float ->
+    binary_float **)
+
+let bdiv prec emax div_nan m x y =
+  let f = fun pl -> B754_nan ((fst pl), (snd pl)) in
+  (match x with
+   | B754_zero sx ->
+     (match y with
+      | B754_infinity sy -> B754_zero (xorb sx sy)
+      | B754_finite (sy, _, _) -> B754_zero (xorb sx sy)
+      | _ -> f (div_nan x y))
+   | B754_infinity sx ->
+     (match y with
+      | B754_zero sy -> B754_infinity (xorb sx sy)
+      | B754_finite (sy, _, _) -> B754_infinity (xorb sx sy)
+      | _ -> f (div_nan x y))
+   | B754_nan (_, _) -> f (div_nan x y)
+   | B754_finite (sx, mx, ex) ->
+     (match y with
+      | B754_zero sy -> B754_infinity (xorb sx sy)
+      | B754_infinity sy -> B754_zero (xorb sx sy)
+      | B754_nan (_, _) -> f (div_nan x y)
+      | B754_finite (sy, my, ey) ->
+        fF2B prec emax
+          (let (p, lz) = fdiv_core_binary prec (Zpos mx) ex (Zpos my) ey in
+           let (mz, ez) = p in
+           (match mz with
+            | Zpos mz0 -> binary_round_aux prec emax m (xorb sx sy) mz0 ez lz
+            | _ -> F754_nan (false, XH)))))
+
+(** val fsqrt_core_binary : z -> z -> z -> (z * z) * location **)
+
+let fsqrt_core_binary prec m e =
+  let d = zdigits2 m in
+  let s = Z.max (Z.sub (Z.mul (Zpos (XO XH)) prec) d) Z0 in
+  let e' = Z.sub e s in
+  if zeven e'
+  then let m' = match s with
+                | Zpos p -> Z.shiftl m (Zpos p)
+                | _ -> m in
+       let (q, r) = Z.sqrtrem m' in
+       let l = if zeq_bool r Z0 then Loc_Exact else Loc_Inexact (if Z.leb r q then Lt else Gt) in
+       ((q, (Z.div2 e')), l)
+  else let s' = Z.add s (Zpos XH) in
+       let e'' = Z.sub e' (Zpos XH) in
+       let m' = match s' with
+                | Zpos p -> Z.shiftl m (Zpos p)
+                | _ -> m in
+       let (q, r) = Z.sqrtrem m' in
+       let l = if zeq_bool r Z0 then Loc_Exact else Loc_Inexact (if Z.leb r q then Lt else Gt) in
+       ((q, (Z.div2 e'')), l)
+
+(** val bsqrt : z -> z -> (binary_float -> bool * nan_pl) -> mode -> binary_float -> binary_float **)
+
+let bsqrt prec emax sqrt_nan m x =
+  let f = fun pl -> B754_nan ((fst pl), (snd pl)) in
+  (match x with
+   | B754_zero _ -> x
+   | B754_infinity b -> if b then f (sqrt_nan x) else x
+   | B754_nan (_, _) -> f (sqrt_nan x)
+   | B754_finite (sx, mx, ex) ->
+     if sx
+     then f (sqrt_nan x)
+     else fF2B prec emax
+            (let (p, lz) = fsqrt_core_binary prec (Zpos mx) ex in
+             let (mz, ez) = p in
+             (match mz with
+              | Zpos mz0 -> binary_round_aux prec emax m false mz0 ez lz
+              | _ -> F754_nan (false, XH))))
+
+type binary64 = binary_float
+
+(** val default_nan_pl64 : bool * nan_pl **)
+
+let default_nan_pl64 =
+  (false,
+    (iter_nat (fun x -> XO x) (S (S (S (S (S (S (S (S (S (S (S (S (S (S (S (S (S (S (S (S (S (S (S (S (S (S
+      (S (S (S (S (S (S (S (S (S (S (S (S (S (S (S (S (S (S (S (S (S (S (S (S (S
+      O))))))))))))))))))))))))))))))))))))))))))))))))))) XH))
+
+(** val unop_nan_pl64 : binary64 -> bool * nan_pl **)
+
+let unop_nan_pl64 = function
+| B754_nan (s, pl) -> (s, pl)
+| _ -> default_nan_pl64
+
+(** val b64_sqrt : mode -> binary_float -> binary_float **)
+
+let b64_sqrt =
+  bsqrt (Zpos (XI (XO (XI (XO (XI XH)))))) (Zpos (XO (XO (XO (XO (XO (XO (XO (XO (XO (XO XH)))))))))))
+    unop_nan_pl64
+
+(** val default_pl_64 : bool * nan_pl **)
+
+let default_pl_64 =
+  (true,
+    (let rec f = function
+     | O -> XH
+     | S n1 -> XO (f n1)
+     in f (S (S (S (S (S (S (S (S (S (S (S (S (S (S (S (S (S (S (S (S (S (S (S (S (S (S (S (S (S (S (S (S (S
+          (S (S (S (S (S (S (S (S (S (S (S (S (S (S (S (S (S (S
+          O)))))))))))))))))))))))))))))))))))))))))))))))))))))
+
+(** val choose_binop_pl_64 : bool -> nan_pl -> bool -> nan_pl -> bool **)
+
+let choose_binop_pl_64 _ _ _ _ =
+  false
+
+type comparison0 =
+| Ceq
+| Cne
+| Clt
+| Cle
+| Cgt
+| Cge
+
+module Wordsize_64 =
+ struct
+  (** val wordsize : nat **)
+
+  let wordsize =
+    S (S (S (S (S (S (S (S (S (S (S (S (S (S (S (S (S (S (S (S (S (S (S (S (S (S (S (S (S (S (S (S (S (S (S
+      (S (S (S (S (S (S (S (S (S (S (S (S (S (S (S (S (S (S (S (S (S (S (S (S (S (S (S (S (S
+      O)))))))))))))))))))))))))))))))))))))))))))))))))))))))))))))))
+ end
+
+module Int64 =
+ struct
+  (** val wordsize : nat **)
+
+  let wordsize =
+    Wordsize_64.wordsize
+
+  (** val modulus : z **)
+
+  let modulus =
+    two_power_nat wordsize
+
+  (** val half_modulus : z **)
+
+  let half_modulus =
+    Z.div modulus (Zpos (XO XH))
+
+  (** val max_signed : z **)
+
+  let max_signed =
+    Z.sub half_modulus (Zpos XH)
+
+  (** val min_signed : z **)
+
+  let min_signed =
+    Z.opp half_modulus
+
+  type int = z
+    (* singleton inductive, whose constructor was mkint *)
+
+  (** val intval : int -> z **)
+
+  let intval i =
+    i
+
+  (** val coq_P_mod_two_p : positive -> nat -> z **)
+
+  let rec coq_P_mod_two_p p = function
+  | O -> Z0
+  | S m ->
+    (match p with
+     | XI q -> Z.succ_double (coq_P_mod_two_p q m)
+     | XO q -> Z.double (coq_P_mod_two_p q m)
+     | XH -> Zpos XH)
+
+  (** val coq_Z_mod_modulus : z -> z **)
+
+  let coq_Z_mod_modulus = function
+  | Z0 -> Z0
+  | Zpos p -> coq_P_mod_two_p p wordsize
+  | Zneg p -> let r = coq_P_mod_two_p p wordsize in if zeq r Z0 then Z0 else Z.sub modulus r
+
+  (** val unsigned : int -> z **)
+
+  let unsigned =
+    intval
+
+  (** val signed : int -> z **)
+
+  let signed n0 =
+    let x = unsigned n0 in if zlt x half_modulus then x else Z.sub x modulus
+
+  (** val repr : z -> int **)
+
+  let repr =
+    coq_Z_mod_modulus
+ end
+
+(** val bofZ : z -> z -> z -> binary_float **)
+
+let bofZ prec emax n0 =
+  binary_normalize prec emax Mode_NE n0 Z0 false
+
+(** val zofB : z -> z -> binary_float -> z option **)
+
+let zofB _ _ = function
+| B754_zero _ -> Some Z0
+| B754_finite (s, m, e0) ->
+  (match e0 with
+   | Z0 -> Some (cond_Zopp s (Zpos m))
+   | Zpos e -> Some (Z.mul (cond_Zopp s (Zpos m)) (Z.pow_pos (radix_val radix2) e))
+   | Zneg e -> Some (cond_Zopp s (Z.div (Zpos m) (Z.pow_pos (radix_val radix2) e))))
+| _ -> None
+
+(** val zofB_range : z -> z -> binary_float -> z -> z -> z option **)
+
+let zofB_range prec emax f zmin zmax =
+  match zofB prec emax f with
+  | Some z0 -> if (&&) (Z.leb zmin z0) (Z.leb z0 zmax) then Some z0 else None
+  | None -> None
+
+(** val pos_pow : positive -> positive -> positive **)
+
+let rec pos_pow x = function
+| XI y0 -> Coq_Pos.mul x (Coq_Pos.square (pos_pow x y0))
+| XO y0 -> Coq_Pos.square (pos_pow x y0)
+| XH -> x
+
+(** val bparse : z -> z -> positive -> positive -> z -> binary_float **)
+
+let bparse prec emax base m e =
+  let emin = Z.sub (Z.sub (Zpos (XI XH)) emax) prec in
+  (match e with
+   | Z0 -> bofZ prec emax (Zpos m)
+   | Zpos p ->
+     if Z.ltb (Z.mul e (Z.log2 (Zpos base))) emax
+     then bofZ prec emax (Z.mul (Zpos m) (Zpos (pos_pow base p)))
+     else B754_infinity false
+   | Zneg p ->
+     if Z.ltb (Z.add (Z.mul e (Z.log2 (Zpos base))) (Z.log2_up (Zpos m))) emin
+     then B754_zero false
+     else fF2B prec emax
+            (let (p0, lz) = fdiv_core_binary prec (Zpos m) Z0 (Zpos (pos_pow base p)) Z0 in
+             let (mz, ez) = p0 in
+             (match mz with
+              | Zpos mz0 -> binary_round_aux prec emax Mode_NE (xorb false false) mz0 ez lz
+              | _ -> F754_nan (false, XH))))
+
+type float = binary64
+
+(** val cmp_of_comparison : comparison0 -> comparison option -> bool **)
+
+let cmp_of_comparison c x =
+  match c with
+  | Ceq -> (match x with
+            | Some c0 -> (match c0 with
+                          | Eq -> true
+                          | _ -> false)
+            | None -> false)
+  | Cne -> (match x with
+            | Some c0 -> (match c0 with
+                          | Eq -> false
+                          | _ -> true)
+            | None -> true)
+  | Clt -> (match x with
+            | Some c0 -> (match c0 with
+                          | Lt -> true
+                          | _ -> false)
+            | None -> false)
+  | Cle -> (match x with
+            | Some c0 -> (match c0 with
+                          | Gt -> false
+                          | _ -> true)
+            | None -> false)
+  | Cgt -> (match x with
+            | Some c0 -> (match c0 with
+                          | Gt -> true
+                          | _ -> false)
+            | None -> false)
+  | Cge -> (match x with
+            | Some c0 -> (match c0 with
+                          | Lt -> false
+                          | _ -> true)
+            | None -> false)
+
+module Float =
+ struct
+  (** val transform_quiet_pl : nan_pl -> nan_pl **)
+
+  let transform_quiet_pl pl =
+    Coq_Pos.coq_lor pl
+      (iter_nat (fun x -> XO x) (S (S (S (S (S (S (S (S (S (S (S (S (S (S (S (S (S (S (S (S (S (S (S (S (S (S
+        (S (S (S (S (S (S (S (S (S (S (S (S (S (S (S (S (S (S (S (S (S (S (S (S (S
+        O))))))))))))))))))))))))))))))))))))))))))))))))))) XH)
+
+  (** val neg_pl : bool -> nan_pl -> bool * nan_pl **)
+
+  let neg_pl s pl =
+    ((negb s), pl)
+
+  (** val abs_pl : bool -> nan_pl -> bool * nan_pl **)
+
+  let abs_pl _ pl =
+    (false, pl)
+
+  (** val binop_pl : binary64 -> binary64 -> bool * nan_pl **)
+
+  let binop_pl x y =
+    match x with
+    | B754_nan (s1, pl1) ->
+      (match y with
+       | B754_nan (s2, pl2) ->
+         if choose_binop_pl_64 s1 pl1 s2 pl2
+         then (s2, (transform_quiet_pl pl2))
+         else (s1, (transform_quiet_pl pl1))
+       | _ -> (s1, (transform_quiet_pl pl1)))
+    | _ -> (match y with
+            | B754_nan (s2, pl2) -> (s2, (transform_quiet_pl pl2))
+            | _ -> default_pl_64)
+
+  (** val zero : float **)
+
+  let zero =
+    B754_zero false
+
+  (** val neg : float -> float **)
+
+  let neg =
+    bopp (Zpos (XI (XO (XI (XO (XI XH)))))) (Zpos (XO (XO (XO (XO (XO (XO (XO (XO (XO (XO XH))))))))))) neg_pl
+
+  (** val abs : float -> float **)
+
+  let abs =
+    babs (Zpos (XI (XO (XI (XO (XI XH)))))) (Zpos (XO (XO (XO (XO (XO (XO (XO (XO (XO (XO XH))))))))))) abs_pl
+
+  (** val add : float -> float -> float **)
+
+  let add =
+    bplus (Zpos (XI (XO (XI (XO (XI XH)))))) (Zpos (XO (XO (XO (XO (XO (XO (XO (XO (XO (XO XH)))))))))))
+      binop_pl Mode_NE
+
+  (** val sub : float -> float -> float **)
+
+  let sub =
+    bminus (Zpos (XI (XO (XI (XO (XI XH)))))) (Zpos (XO (XO (XO (XO (XO (XO (XO (XO (XO (XO XH)))))))))))
+      binop_pl Mode_NE
+
+  (** val mul : float -> float -> float **)
+
+  let mul =
+    bmult (Zpos (XI (XO (XI (XO (XI XH)))))) (Zpos (XO (XO (XO (XO (XO (XO (XO (XO (XO (XO XH)))))))))))
+      binop_pl Mode_NE
+
+  (** val div : float -> float -> float **)
+
+  let div =
+    bdiv (Zpos (XI (XO (XI (XO (XI XH)))))) (Zpos (XO (XO (XO (XO (XO (XO (XO (XO (XO (XO XH)))))))))))
+      binop_pl Mode_NE
+
+  (** val compare : float -> float -> comparison option **)
+
+  let compare f1 f2 =
+    bcompare (Zpos (XI (XO (XI (XO (XI XH)))))) (Zpos (XO (XO (XO (XO (XO (XO (XO (XO (XO (XO XH)))))))))))
+      f1 f2
+
+  (** val cmp : comparison0 -> float -> float -> bool **)
+
+  let cmp c f1 f2 =
+    cmp_of_comparison c (compare f1 f2)
+
+  (** val to_long : float -> Int64.int option **)
+
+  let to_long f =
+    option_map Int64.repr
+      (zofB_range (Zpos (XI (XO (XI (XO (XI XH)))))) (Zpos (XO (XO (XO (XO (XO (XO (XO (XO (XO (XO
+        XH))))))))))) f Int64.min_signed Int64.max_signed)
+
+  (** val from_parsed : positive -> positive -> z -> float **)
+
+  let from_parsed base intPart expPart =
+    bparse (Zpos (XI (XO (XI (XO (XI XH)))))) (Zpos (XO (XO (XO (XO (XO (XO (XO (XO (XO (XO XH)))))))))))
+      base intPart expPart
+ end
+
+type 'm monadOps = { bind : (__ -> __ -> 'm -> (__ -> 'm) -> 'm); ret : (__ -> __ -> 'm) }
+
+(** val bind : 'a1 monadOps -> 'a1 -> ('a2 -> 'a1) -> 'a1 **)
+
+let bind monadOps0 x x0 =
+  let { bind = bind0; ret = _ } = monadOps0 in Obj.magic bind0 __ __ x x0
+
+(** val ret : 'a1 monadOps -> 'a2 -> 'a1 **)
+
+let ret monadOps0 x =
+  let { bind = _; ret = ret0 } = monadOps0 in Obj.magic ret0 __ x
+
+type 't monadTransformerOps = { tops : (__ -> __ monadOps -> 't monadOps);
+                                lift : (__ -> __ monadOps -> __ -> __ -> 't) }
+
+(** val tops : 'a1 monadTransformerOps -> 'a2 monadOps -> 'a1 monadOps **)
+
+let tops monadTransformerOps0 h =
+  let { tops = tops0; lift = _ } = monadTransformerOps0 in Obj.magic tops0 __ h
+
+(** val idM : __ monadOps **)
+
+let idM =
+  { bind = (fun _ _ x f -> f x); ret = (fun _ x -> x) }
+
+(** val monad_of_transformer : 'a1 monadTransformerOps -> 'a1 monadOps **)
+
+let monad_of_transformer h =
+  tops h idM
+
+(** val optionT : __ monadTransformerOps **)
+
+let optionT =
+  { tops = (fun _ h -> { bind = (fun _ _ x f ->
+    bind h x (fun a -> match a with
+                       | Some a' -> f a'
+                       | None -> ret h None)); ret = (fun _ x -> ret h (Some x)) }); lift = (fun _ h _ x ->
+    bind h x (fun a -> ret h (Some a))) }
+
+(** val optionM : __ option monadOps **)
+
+let optionM =
+  monad_of_transformer (Obj.magic optionT)
+
+module FloatIO =
+ struct
+  (** val coq_Z_to_float : z -> float **)
+
+  let coq_Z_to_float = function
+  | Z0 -> Float.zero
+  | Zpos x -> Float.from_parsed (XO (XI (XO XH))) x Z0
+  | Zneg x -> Float.neg (Float.from_parsed (XO (XI (XO XH))) x Z0)
+
+  module Details =
+   struct
+    (** val precision_of_float : z **)
+
+    let precision_of_float =
+      Zpos (XI (XO (XI (XO (XI XH)))))
+
+    (** val log10of2scaled3 : z **)
+
+    let log10of2scaled3 =
+      Zpos (XI (XO (XI (XI (XO (XI (XO (XO XH))))))))
+
+    (** val strToUintHelper : char list -> uint option **)
+
+    let rec strToUintHelper = function
+    | [] -> Some Nil
+    | x::x0 ->
+      bind (Obj.magic optionM) (strToUintHelper x0) (fun lower ->
+        (* If this appears, you're using Ascii internals. Please don't *)
+ (fun f c ->
+  let n = Char.code c in
+  let h i = (n land (1 lsl i)) <> 0 in
+  f (h 0) (h 1) (h 2) (h 3) (h 4) (h 5) (h 6) (h 7))
+          (fun b b0 b1 b2 b3 b4 b5 b6 ->
+          if b
+          then if b0
+               then if b1
+                    then if b2
+                         then None
+                         else if b3
+                              then if b4
+                                   then if b5 then None else if b6 then None else Some (D7 lower)
+                                   else None
+                              else None
+                    else if b2
+                         then None
+                         else if b3
+                              then if b4
+                                   then if b5 then None else if b6 then None else Some (D3 lower)
+                                   else None
+                              else None
+               else if b1
+                    then if b2
+                         then None
+                         else if b3
+                              then if b4
+                                   then if b5 then None else if b6 then None else Some (D5 lower)
+                                   else None
+                              else None
+                    else if b2
+                         then if b3
+                              then if b4
+                                   then if b5 then None else if b6 then None else Some (D9 lower)
+                                   else None
+                              else None
+                         else if b3
+                              then if b4
+                                   then if b5 then None else if b6 then None else Some (D1 lower)
+                                   else None
+                              else None
+          else if b0
+               then if b1
+                    then if b2
+                         then None
+                         else if b3
+                              then if b4
+                                   then if b5 then None else if b6 then None else Some (D6 lower)
+                                   else None
+                              else None
+                    else if b2
+                         then None
+                         else if b3
+                              then if b4
+                                   then if b5 then None else if b6 then None else Some (D2 lower)
+                                   else None
+                              else None
+               else if b1
+                    then if b2
+                         then None
+                         else if b3
+                              then if b4
+                                   then if b5 then None else if b6 then None else Some (D4 lower)
+                                   else None
+                              else None
+                    else if b2
+                         then if b3
+                              then if b4
+                                   then if b5 then None else if b6 then None else Some (D8 lower)
+                                   else None
+                              else None
+                         else if b3
+                              then if b4
+                                   then if b5 then None else if b6 then None else Some (D0 lower)
+                                   else None
+                              else None)
+          x)
+
+    (** val strToUint : char list -> uint option **)
+
+    let strToUint s =
+      bind (Obj.magic optionM) (strToUintHelper s) (fun x -> Some (unorm x))
+
+    (** val strToIntHelper : char list -> int option **)
+
+    let strToIntHelper s = match s with
+    | [] -> Some (Pos (D0 Nil))
+    | x::x0 ->
+      (* If this appears, you're using Ascii internals. Please don't *)
+ (fun f c ->
+  let n = Char.code c in
+  let h i = (n land (1 lsl i)) <> 0 in
+  f (h 0) (h 1) (h 2) (h 3) (h 4) (h 5) (h 6) (h 7))
+        (fun b b0 b1 b2 b3 b4 b5 b6 ->
+        if b
+        then if b0
+             then if b1
+                  then let sign = false in
+                       bind (Obj.magic optionM) (Obj.magic strToUint s) (fun uintVal -> Some
+                         (if sign then Neg uintVal else Pos uintVal))
+                  else if b2
+                       then if b3
+                            then let sign = false in
+                                 bind (Obj.magic optionM) (Obj.magic strToUint s) (fun uintVal -> Some
+                                   (if sign then Neg uintVal else Pos uintVal))
+                            else if b4
+                                 then if b5
+                                      then let sign = false in
+                                           bind (Obj.magic optionM) (Obj.magic strToUint s) (fun uintVal ->
+                                             Some (if sign then Neg uintVal else Pos uintVal))
+                                      else if b6
+                                           then let sign = false in
+                                                bind (Obj.magic optionM) (Obj.magic strToUint s)
+                                                  (fun uintVal -> Some
+                                                  (if sign then Neg uintVal else Pos uintVal))
+                                           else let sign = false in
+                                                bind (Obj.magic optionM) (Obj.magic strToUint x0)
+                                                  (fun uintVal -> Some
+                                                  (if sign then Neg uintVal else Pos uintVal))
+                                 else let sign = false in
+                                      bind (Obj.magic optionM) (Obj.magic strToUint s) (fun uintVal -> Some
+                                        (if sign then Neg uintVal else Pos uintVal))
+                       else let sign = false in
+                            bind (Obj.magic optionM) (Obj.magic strToUint s) (fun uintVal -> Some
+                              (if sign then Neg uintVal else Pos uintVal))
+             else if b1
+                  then if b2
+                       then if b3
+                            then let sign = false in
+                                 bind (Obj.magic optionM) (Obj.magic strToUint s) (fun uintVal -> Some
+                                   (if sign then Neg uintVal else Pos uintVal))
+                            else if b4
+                                 then if b5
+                                      then let sign = false in
+                                           bind (Obj.magic optionM) (Obj.magic strToUint s) (fun uintVal ->
+                                             Some (if sign then Neg uintVal else Pos uintVal))
+                                      else if b6
+                                           then let sign = false in
+                                                bind (Obj.magic optionM) (Obj.magic strToUint s)
+                                                  (fun uintVal -> Some
+                                                  (if sign then Neg uintVal else Pos uintVal))
+                                           else let sign = true in
+                                                bind (Obj.magic optionM) (Obj.magic strToUint x0)
+                                                  (fun uintVal -> Some
+                                                  (if sign then Neg uintVal else Pos uintVal))
+                                 else let sign = false in
+                                      bind (Obj.magic optionM) (Obj.magic strToUint s) (fun uintVal -> Some
+                                        (if sign then Neg uintVal else Pos uintVal))
+                       else let sign = false in
+                            bind (Obj.magic optionM) (Obj.magic strToUint s) (fun uintVal -> Some
+                              (if sign then Neg uintVal else Pos uintVal))
+                  else let sign = false in
+                       bind (Obj.magic optionM) (Obj.magic strToUint s) (fun uintVal -> Some
+                         (if sign then Neg uintVal else Pos uintVal))
+        else let sign = false in
+             bind (Obj.magic optionM) (Obj.magic strToUint s) (fun uintVal -> Some
+               (if sign then Neg uintVal else Pos uintVal)))
+        x
+
+    (** val strToInt : char list -> int option **)
+
+    let strToInt s =
+      bind (Obj.magic optionM) (strToIntHelper s) (fun x -> Some (norm x))
+
+    (** val strToZ : char list -> z option **)
+
+    let strToZ s =
+      bind (Obj.magic optionM) (Obj.magic strToInt s) (fun x -> Some (Z.of_int x))
+
+    (** val splitAtExponent : char list -> char list * char list **)
+
+    let splitAtExponent s =
+      let maybeEpos = match index O ('E'::[]) s with
+                      | Some epos -> Some epos
+                      | None -> index O ('e'::[]) s in
+      (match maybeEpos with
+       | Some epos -> ((substring O epos s), (substring (S epos) (sub (sub (length s) epos) (S O)) s))
+       | None -> (s, []))
+
+    (** val splitAtPoint : char list -> char list * char list **)
+
+    let splitAtPoint s =
+      match index O ('.'::[]) s with
+      | Some dpos -> ((substring O dpos s), (substring (S dpos) (sub (sub (length s) dpos) (S O)) s))
+      | None -> (s, [])
+
+    (** val decomposeFloatString : char list -> (char list * char list) * char list **)
+
+    let decomposeFloatString s =
+      let (frac, exp) = splitAtExponent s in ((splitAtPoint frac), exp)
+
+    (** val strToFloatHelper : char list -> (z * z) option **)
+
+    let strToFloatHelper s =
+      let (p, exp) = decomposeFloatString s in
+      let (intPart, fracPart) = p in
+      let mantstring = append intPart fracPart in
+      bind (Obj.magic optionM) (Obj.magic strToZ mantstring) (fun zmant ->
+        bind (Obj.magic optionM) (Obj.magic strToZ exp) (fun zexp ->
+          let adjustedZexp = Z.sub zexp (Z.of_nat (length fracPart)) in
+          ret (Obj.magic optionM) (zmant, adjustedZexp)))
+
+    (** val strToFloat : char list -> float option **)
+
+    let strToFloat s =
+      match strToFloatHelper s with
+      | Some p ->
+        let (zmant, adjustedZexp) = p in
+        ret (Obj.magic optionM)
+          (match zmant with
+           | Z0 -> Float.zero
+           | Zpos x -> Float.from_parsed (XO (XI (XO XH))) x adjustedZexp
+           | Zneg x -> Float.neg (Float.from_parsed (XO (XI (XO XH))) x adjustedZexp))
+      | None -> None
+
+    (** val scale_exp : z -> z -> z **)
+
+    let scale_exp d e =
+      Z.sub (Z.sub d (Zpos (XO XH)))
+        (Z.div (Z.mul (Z.sub (Z.add e precision_of_float) (Zpos XH)) log10of2scaled3) (Zpos (XO (XO (XO (XI
+          (XO (XI (XI (XI (XI XH)))))))))))
+
+    (** val digits : z -> char list **)
+
+    let digits = function
+    | Z0 -> '0'::[]
+    | Zpos p ->
+      (match p with
+       | XI p0 ->
+         (match p0 with
+          | XI p1 ->
+            (match p1 with
+             | XI p2 ->
+               (match p2 with
+                | XI p3 ->
+                  (match p3 with
+                   | XH -> 'v'::[]
+                   | _ ->
+                     '!'::(' '::('E'::('r'::('r'::('o'::('r'::('.'::(' '::('M'::('a'::('x'::(' '::('r'::('a'::('d'::('i'::('x'::(' '::('i'::('s'::(' '::('3'::('5'::(' '::('!'::[]))))))))))))))))))))))))))
+                | XO p3 ->
+                  (match p3 with
+                   | XH -> 'n'::[]
+                   | _ ->
+                     '!'::(' '::('E'::('r'::('r'::('o'::('r'::('.'::(' '::('M'::('a'::('x'::(' '::('r'::('a'::('d'::('i'::('x'::(' '::('i'::('s'::(' '::('3'::('5'::(' '::('!'::[]))))))))))))))))))))))))))
+                | XH -> 'f'::[])
+             | XO p2 ->
+               (match p2 with
+                | XI p3 ->
+                  (match p3 with
+                   | XH -> 'r'::[]
+                   | _ ->
+                     '!'::(' '::('E'::('r'::('r'::('o'::('r'::('.'::(' '::('M'::('a'::('x'::(' '::('r'::('a'::('d'::('i'::('x'::(' '::('i'::('s'::(' '::('3'::('5'::(' '::('!'::[]))))))))))))))))))))))))))
+                | XO p3 ->
+                  (match p3 with
+                   | XI _ ->
+                     '!'::(' '::('E'::('r'::('r'::('o'::('r'::('.'::(' '::('M'::('a'::('x'::(' '::('r'::('a'::('d'::('i'::('x'::(' '::('i'::('s'::(' '::('3'::('5'::(' '::('!'::[])))))))))))))))))))))))))
+                   | XO p4 ->
+                     (match p4 with
+                      | XH -> 'z'::[]
+                      | _ ->
+                        '!'::(' '::('E'::('r'::('r'::('o'::('r'::('.'::(' '::('M'::('a'::('x'::(' '::('r'::('a'::('d'::('i'::('x'::(' '::('i'::('s'::(' '::('3'::('5'::(' '::('!'::[]))))))))))))))))))))))))))
+                   | XH -> 'j'::[])
+                | XH -> 'b'::[])
+             | XH -> '7'::[])
+          | XO p1 ->
+            (match p1 with
+             | XI p2 ->
+               (match p2 with
+                | XI p3 ->
+                  (match p3 with
+                   | XH -> 't'::[]
+                   | _ ->
+                     '!'::(' '::('E'::('r'::('r'::('o'::('r'::('.'::(' '::('M'::('a'::('x'::(' '::('r'::('a'::('d'::('i'::('x'::(' '::('i'::('s'::(' '::('3'::('5'::(' '::('!'::[]))))))))))))))))))))))))))
+                | XO p3 ->
+                  (match p3 with
+                   | XH -> 'l'::[]
+                   | _ ->
+                     '!'::(' '::('E'::('r'::('r'::('o'::('r'::('.'::(' '::('M'::('a'::('x'::(' '::('r'::('a'::('d'::('i'::('x'::(' '::('i'::('s'::(' '::('3'::('5'::(' '::('!'::[]))))))))))))))))))))))))))
+                | XH -> 'd'::[])
+             | XO p2 ->
+               (match p2 with
+                | XI p3 ->
+                  (match p3 with
+                   | XH -> 'p'::[]
+                   | _ ->
+                     '!'::(' '::('E'::('r'::('r'::('o'::('r'::('.'::(' '::('M'::('a'::('x'::(' '::('r'::('a'::('d'::('i'::('x'::(' '::('i'::('s'::(' '::('3'::('5'::(' '::('!'::[]))))))))))))))))))))))))))
+                | XO p3 ->
+                  (match p3 with
+                   | XI _ ->
+                     '!'::(' '::('E'::('r'::('r'::('o'::('r'::('.'::(' '::('M'::('a'::('x'::(' '::('r'::('a'::('d'::('i'::('x'::(' '::('i'::('s'::(' '::('3'::('5'::(' '::('!'::[])))))))))))))))))))))))))
+                   | XO p4 ->
+                     (match p4 with
+                      | XH -> 'x'::[]
+                      | _ ->
+                        '!'::(' '::('E'::('r'::('r'::('o'::('r'::('.'::(' '::('M'::('a'::('x'::(' '::('r'::('a'::('d'::('i'::('x'::(' '::('i'::('s'::(' '::('3'::('5'::(' '::('!'::[]))))))))))))))))))))))))))
+                   | XH -> 'h'::[])
+                | XH -> '9'::[])
+             | XH -> '5'::[])
+          | XH -> '3'::[])
+       | XO p0 ->
+         (match p0 with
+          | XI p1 ->
+            (match p1 with
+             | XI p2 ->
+               (match p2 with
+                | XI p3 ->
+                  (match p3 with
+                   | XH -> 'u'::[]
+                   | _ ->
+                     '!'::(' '::('E'::('r'::('r'::('o'::('r'::('.'::(' '::('M'::('a'::('x'::(' '::('r'::('a'::('d'::('i'::('x'::(' '::('i'::('s'::(' '::('3'::('5'::(' '::('!'::[]))))))))))))))))))))))))))
+                | XO p3 ->
+                  (match p3 with
+                   | XH -> 'm'::[]
+                   | _ ->
+                     '!'::(' '::('E'::('r'::('r'::('o'::('r'::('.'::(' '::('M'::('a'::('x'::(' '::('r'::('a'::('d'::('i'::('x'::(' '::('i'::('s'::(' '::('3'::('5'::(' '::('!'::[]))))))))))))))))))))))))))
+                | XH -> 'e'::[])
+             | XO p2 ->
+               (match p2 with
+                | XI p3 ->
+                  (match p3 with
+                   | XH -> 'q'::[]
+                   | _ ->
+                     '!'::(' '::('E'::('r'::('r'::('o'::('r'::('.'::(' '::('M'::('a'::('x'::(' '::('r'::('a'::('d'::('i'::('x'::(' '::('i'::('s'::(' '::('3'::('5'::(' '::('!'::[]))))))))))))))))))))))))))
+                | XO p3 ->
+                  (match p3 with
+                   | XI _ ->
+                     '!'::(' '::('E'::('r'::('r'::('o'::('r'::('.'::(' '::('M'::('a'::('x'::(' '::('r'::('a'::('d'::('i'::('x'::(' '::('i'::('s'::(' '::('3'::('5'::(' '::('!'::[])))))))))))))))))))))))))
+                   | XO p4 ->
+                     (match p4 with
+                      | XH -> 'y'::[]
+                      | _ ->
+                        '!'::(' '::('E'::('r'::('r'::('o'::('r'::('.'::(' '::('M'::('a'::('x'::(' '::('r'::('a'::('d'::('i'::('x'::(' '::('i'::('s'::(' '::('3'::('5'::(' '::('!'::[]))))))))))))))))))))))))))
+                   | XH -> 'i'::[])
+                | XH -> 'a'::[])
+             | XH -> '6'::[])
+          | XO p1 ->
+            (match p1 with
+             | XI p2 ->
+               (match p2 with
+                | XI p3 ->
+                  (match p3 with
+                   | XH -> 's'::[]
+                   | _ ->
+                     '!'::(' '::('E'::('r'::('r'::('o'::('r'::('.'::(' '::('M'::('a'::('x'::(' '::('r'::('a'::('d'::('i'::('x'::(' '::('i'::('s'::(' '::('3'::('5'::(' '::('!'::[]))))))))))))))))))))))))))
+                | XO p3 ->
+                  (match p3 with
+                   | XH -> 'k'::[]
+                   | _ ->
+                     '!'::(' '::('E'::('r'::('r'::('o'::('r'::('.'::(' '::('M'::('a'::('x'::(' '::('r'::('a'::('d'::('i'::('x'::(' '::('i'::('s'::(' '::('3'::('5'::(' '::('!'::[]))))))))))))))))))))))))))
+                | XH -> 'c'::[])
+             | XO p2 ->
+               (match p2 with
+                | XI p3 ->
+                  (match p3 with
+                   | XH -> 'o'::[]
+                   | _ ->
+                     '!'::(' '::('E'::('r'::('r'::('o'::('r'::('.'::(' '::('M'::('a'::('x'::(' '::('r'::('a'::('d'::('i'::('x'::(' '::('i'::('s'::(' '::('3'::('5'::(' '::('!'::[]))))))))))))))))))))))))))
+                | XO p3 ->
+                  (match p3 with
+                   | XI _ ->
+                     '!'::(' '::('E'::('r'::('r'::('o'::('r'::('.'::(' '::('M'::('a'::('x'::(' '::('r'::('a'::('d'::('i'::('x'::(' '::('i'::('s'::(' '::('3'::('5'::(' '::('!'::[])))))))))))))))))))))))))
+                   | XO p4 ->
+                     (match p4 with
+                      | XH -> 'w'::[]
+                      | _ ->
+                        '!'::(' '::('E'::('r'::('r'::('o'::('r'::('.'::(' '::('M'::('a'::('x'::(' '::('r'::('a'::('d'::('i'::('x'::(' '::('i'::('s'::(' '::('3'::('5'::(' '::('!'::[]))))))))))))))))))))))))))
+                   | XH -> 'g'::[])
+                | XH -> '8'::[])
+             | XH -> '4'::[])
+          | XH -> '2'::[])
+       | XH -> '1'::[])
+    | Zneg _ ->
+      '!'::(' '::('E'::('r'::('r'::('o'::('r'::('.'::(' '::('M'::('a'::('x'::(' '::('r'::('a'::('d'::('i'::('x'::(' '::('i'::('s'::(' '::('3'::('5'::(' '::('!'::[])))))))))))))))))))))))))
+
+    (** val repeat_string : nat -> char list -> char list **)
+
+    let rec repeat_string n0 c =
+      match n0 with
+      | O -> []
+      | S x -> append c (repeat_string x c)
+
+    (** val coq_Z_to_string_base10_aux : nat -> nat -> z -> char list **)
+
+    let rec coq_Z_to_string_base10_aux min_digits fuel num =
+      if Z.ltb num Z0
+      then 'R'::('e'::('q'::('u'::('i'::('r'::('e'::(' '::('n'::('o'::('n'::('-'::('n'::('e'::('g'::('a'::('t'::('i'::('v'::('e'::(' '::('n'::('u'::('m'::('.'::[]))))))))))))))))))))))))
+      else (match fuel with
+            | O -> 'o'::('u'::('t'::(' '::('o'::('f'::(' '::('f'::('u'::('e'::('l'::[]))))))))))
+            | S x ->
+              (match num with
+               | Z0 -> repeat_string min_digits ('0'::[])
+               | _ ->
+                 append (coq_Z_to_string_base10_aux (pred min_digits) x (Z.div num (Zpos (XO (XI (XO XH))))))
+                   (digits (Z.modulo num (Zpos (XO (XI (XO XH))))))))
+
+    (** val coq_Z_to_string_base10 : nat -> z -> char list **)
+
+    let coq_Z_to_string_base10 min_digits num =
+      if Z.ltb num Z0
+      then append ('-'::[])
+             (coq_Z_to_string_base10_aux min_digits (S (S (S (S (S (S (S (S (S (S (S (S (S (S (S (S (S (S (S
+               (S (S (S (S (S (S (S (S (S (S (S (S (S (S (S (S (S (S (S (S (S (S (S (S (S (S (S (S (S (S (S
+               (S (S (S (S (S (S (S (S (S (S (S (S (S (S (S (S (S (S (S (S (S (S (S (S (S (S (S (S (S (S (S
+               (S (S (S (S (S (S (S (S (S (S (S (S (S (S (S (S (S (S (S
+               O))))))))))))))))))))))))))))))))))))))))))))))))))))))))))))))))))))))))))))))))))))))))))))))))))))
+               (Z.opp num))
+      else if Z.eqb num Z0
+           then repeat_string min_digits ('0'::[])
+           else coq_Z_to_string_base10_aux min_digits (S (S (S (S (S (S (S (S (S (S (S (S (S (S (S (S (S (S
+                  (S (S (S (S (S (S (S (S (S (S (S (S (S (S (S (S (S (S (S (S (S (S (S (S (S (S (S (S (S (S
+                  (S (S (S (S (S (S (S (S (S (S (S (S (S (S (S (S (S (S (S (S (S (S (S (S (S (S (S (S (S (S
+                  (S (S (S (S (S (S (S (S (S (S (S (S (S (S (S (S (S (S (S (S (S (S
+                  O))))))))))))))))))))))))))))))))))))))))))))))))))))))))))))))))))))))))))))))))))))))))))))))))))))
+                  num
+
+    (** val scaled_float_to_Z : float -> z -> z **)
+
+    let scaled_float_to_Z x fdigs0 =
+      match Float.to_long (Float.mul x (Float.from_parsed (XO (XI (XO XH))) XH fdigs0)) with
+      | Some ii -> Int64.signed ii
+      | None -> Z0
+
+    (** val insert_decimal : char list -> nat -> char list **)
+
+    let insert_decimal s fdigs0 =
+      let len = length s in
+      let front = sub len fdigs0 in append (substring O front s) (append ('.'::[]) (substring front fdigs0 s))
+
+    (** val float_to_string_unsigned : float -> nat -> char list **)
+
+    let float_to_string_unsigned x fdigs0 =
+      match x with
+      | B754_finite (b, _, e) ->
+        if b
+        then []
+        else let digs_after_dec = pred fdigs0 in
+             let scale = scale_exp (Z.of_nat fdigs0) e in
+             let scaled = scaled_float_to_Z x scale in
+             let b10 = coq_Z_to_string_base10 (S O) scaled in
+             let lb10 = length b10 in
+             let scale' = if Nat.ltb lb10 fdigs0 then Z.add scale (Z.of_nat (sub fdigs0 lb10)) else scale in
+             let b10' =
+               if Nat.ltb lb10 fdigs0
+               then let scaled' = scaled_float_to_Z x scale' in coq_Z_to_string_base10 fdigs0 scaled'
+               else b10
+             in
+             let d10 = insert_decimal b10' digs_after_dec in
+             let true_exp = Z.sub (Z.sub (Z.of_nat fdigs0) scale') (Zpos XH) in
+             let exp_string = coq_Z_to_string_base10 (S O) true_exp in
+             append d10 (append ('e'::[]) exp_string)
+      | _ -> []
+
+    (** val float_to_string_unpadded : float -> nat -> char list **)
+
+    let float_to_string_unpadded x fdigs0 =
+      match x with
+      | B754_zero b -> if b then '-'::('0'::('.'::('0'::[]))) else '0'::('.'::('0'::[]))
+      | B754_infinity b -> if b then '-'::('i'::('n'::('f'::[]))) else 'i'::('n'::('f'::[]))
+      | B754_nan (b, _) -> if b then '-'::('n'::('a'::('n'::[]))) else 'n'::('a'::('n'::[]))
+      | B754_finite (b, _, _) ->
+        if b
+        then append ('-'::[]) (float_to_string_unsigned (Float.abs x) fdigs0)
+        else float_to_string_unsigned x fdigs0
+
+    (** val pad_to_width : nat -> char list -> char list **)
+
+    let pad_to_width width0 s =
+      let ls = length s in let pads = repeat_string (sub width0 ls) (' '::[]) in append pads s
+
+    (** val float_to_string : nat -> nat -> float -> char list **)
+
+    let float_to_string width0 fdigs0 x =
+      pad_to_width width0 (float_to_string_unpadded x fdigs0)
+   end
+
+  (** val coq_Z_to_string_base10 : nat -> z -> char list **)
+
+  let coq_Z_to_string_base10 =
+    Details.coq_Z_to_string_base10
+
+  (** val float_to_string : nat -> nat -> float -> char list **)
+
+  let float_to_string =
+    Details.float_to_string
+
+  (** val strToFloat : char list -> float option **)
+
+  let strToFloat =
+    Details.strToFloat
+
+  (** val strToFloat' : char list -> float **)
+
+  let strToFloat' s =
+    match strToFloat s with
+    | Some x -> x
+    | None -> Float.zero
+ end
+
+module DebugIO =
+ struct
+  (** val width : nat **)
+
+  let width =
+    S (S (S (S (S (S (S (S (S (S (S (S (S (S O)))))))))))))
+
+  (** val fdigs : nat **)
+
+  let fdigs =
+    S (S (S (S (S (S (S (S (S O))))))))
+
+  (** val print_float : float -> char list **)
+
+  let print_float =
+    FloatIO.float_to_string width fdigs
+
+  (** val print_Z : z -> char list **)
+
+  let print_Z =
+    FloatIO.coq_Z_to_string_base10 (S O)
+ end
+
+module PTree =
+ struct
+  type 'a tree =
+  | Leaf
+  | Node of 'a tree * 'a option * 'a tree
+
+  type 'a t = 'a tree
+
+  (** val empty : 'a1 t **)
+
+  let empty =
+    Leaf
+
+  (** val get : positive -> 'a1 t -> 'a1 option **)
+
+  let rec get i = function
+  | Leaf -> None
+  | Node (l, o, r) -> (match i with
+                       | XI ii -> get ii r
+                       | XO ii -> get ii l
+                       | XH -> o)
+
+  (** val set : positive -> 'a1 -> 'a1 t -> 'a1 t **)
+
+  let rec set i v = function
+  | Leaf ->
+    (match i with
+     | XI ii -> Node (Leaf, None, (set ii v Leaf))
+     | XO ii -> Node ((set ii v Leaf), None, Leaf)
+     | XH -> Node (Leaf, (Some v), Leaf))
+  | Node (l, o, r) ->
+    (match i with
+     | XI ii -> Node (l, o, (set ii v r))
+     | XO ii -> Node ((set ii v l), o, r)
+     | XH -> Node (l, (Some v), r))
+
+  (** val remove : positive -> 'a1 t -> 'a1 t **)
+
+  let rec remove i m =
+    match i with
+    | XI ii ->
+      (match m with
+       | Leaf -> Leaf
+       | Node (l, o, r) ->
+         (match l with
+          | Leaf ->
+            (match o with
+             | Some _ -> Node (l, o, (remove ii r))
+             | None ->
+               (match remove ii r with
+                | Leaf -> Leaf
+                | Node (t0, o0, t1) -> Node (Leaf, None, (Node (t0, o0, t1)))))
+          | Node (_, _, _) -> Node (l, o, (remove ii r))))
+    | XO ii ->
+      (match m with
+       | Leaf -> Leaf
+       | Node (l, o, r) ->
+         (match o with
+          | Some _ -> Node ((remove ii l), o, r)
+          | None ->
+            (match r with
+             | Leaf ->
+               (match remove ii l with
+                | Leaf -> Leaf
+                | Node (t0, o0, t1) -> Node ((Node (t0, o0, t1)), None, Leaf))
+             | Node (_, _, _) -> Node ((remove ii l), o, r))))
+    | XH ->
+      (match m with
+       | Leaf -> Leaf
+       | Node (l, _, r) ->
+         (match l with
+          | Leaf -> (match r with
+                     | Leaf -> Leaf
+                     | Node (_, _, _) -> Node (l, None, r))
+          | Node (_, _, _) -> Node (l, None, r)))
+
+  (** val bempty : 'a1 t -> bool **)
+
+  let rec bempty = function
+  | Leaf -> true
+  | Node (l, o, r) -> (match o with
+                       | Some _ -> false
+                       | None -> (&&) (bempty l) (bempty r))
+
+  (** val beq : ('a1 -> 'a1 -> bool) -> 'a1 t -> 'a1 t -> bool **)
+
+  let rec beq beqA m1 m2 =
+    match m1 with
+    | Leaf -> bempty m2
+    | Node (l1, o1, r1) ->
+      (match m2 with
+       | Leaf -> bempty m1
+       | Node (l2, o2, r2) ->
+         (&&)
+           ((&&)
+             (match o1 with
+              | Some y1 -> (match o2 with
+                            | Some y2 -> beqA y1 y2
+                            | None -> false)
+              | None -> (match o2 with
+                         | Some _ -> false
+                         | None -> true)) (beq beqA l1 l2)) (beq beqA r1 r2))
+
+  (** val prev_append : positive -> positive -> positive **)
+
+  let rec prev_append i j =
+    match i with
+    | XI i' -> prev_append i' (XI j)
+    | XO i' -> prev_append i' (XO j)
+    | XH -> j
+
+  (** val prev : positive -> positive **)
+
+  let prev i =
+    prev_append i XH
+
+  (** val coq_Node' : 'a1 t -> 'a1 option -> 'a1 t -> 'a1 t **)
+
+  let coq_Node' l x r =
+    match l with
+    | Leaf ->
+      (match x with
+       | Some _ -> Node (l, x, r)
+       | None -> (match r with
+                  | Leaf -> Leaf
+                  | Node (_, _, _) -> Node (l, x, r)))
+    | Node (_, _, _) -> Node (l, x, r)
+
+  (** val xcombine_l : ('a1 option -> 'a2 option -> 'a3 option) -> 'a1 t -> 'a3 t **)
+
+  let rec xcombine_l f = function
+  | Leaf -> Leaf
+  | Node (l, o, r) -> coq_Node' (xcombine_l f l) (f o None) (xcombine_l f r)
+
+  (** val xcombine_r : ('a1 option -> 'a2 option -> 'a3 option) -> 'a2 t -> 'a3 t **)
+
+  let rec xcombine_r f = function
+  | Leaf -> Leaf
+  | Node (l, o, r) -> coq_Node' (xcombine_r f l) (f None o) (xcombine_r f r)
+
+  (** val combine : ('a1 option -> 'a2 option -> 'a3 option) -> 'a1 t -> 'a2 t -> 'a3 t **)
+
+  let rec combine f m1 m2 =
+    match m1 with
+    | Leaf -> xcombine_r f m2
+    | Node (l1, o1, r1) ->
+      (match m2 with
+       | Leaf -> xcombine_l f m1
+       | Node (l2, o2, r2) -> coq_Node' (combine f l1 l2) (f o1 o2) (combine f r1 r2))
+
+  (** val xelements : 'a1 t -> positive -> (positive * 'a1) list -> (positive * 'a1) list **)
+
+  let rec xelements m i k =
+    match m with
+    | Leaf -> k
+    | Node (l, o, r) ->
+      (match o with
+       | Some x -> xelements l (XO i) (((prev i), x) :: (xelements r (XI i) k))
+       | None -> xelements l (XO i) (xelements r (XI i) k))
+
+  (** val elements : 'a1 t -> (positive * 'a1) list **)
+
+  let elements m =
+    xelements m XH []
+ end
+
+module type INDEXED_TYPE =
+ sig
+  type t
+
+  val index : t -> positive
+
+  val eq : t -> t -> bool
+ end
+
+module ITree =
+ functor (X:INDEXED_TYPE) ->
+ struct
+  type elt = X.t
+
+  (** val elt_eq : X.t -> X.t -> bool **)
+
+  let elt_eq =
+    X.eq
+
+  type 'x t = 'x PTree.t
+
+  (** val empty : 'a1 t **)
+
+  let empty =
+    PTree.empty
+
+  (** val get : elt -> 'a1 t -> 'a1 option **)
+
+  let get k m =
+    PTree.get (X.index k) m
+
+  (** val set : elt -> 'a1 -> 'a1 t -> 'a1 t **)
+
+  let set k v m =
+    PTree.set (X.index k) v m
+
+  (** val remove : elt -> 'a1 t -> 'a1 t **)
+
+  let remove k m =
+    PTree.remove (X.index k) m
+
+  (** val beq : ('a1 -> 'a1 -> bool) -> 'a1 t -> 'a1 t -> bool **)
+
+  let beq =
+    PTree.beq
+
+  (** val combine : ('a1 option -> 'a2 option -> 'a3 option) -> 'a1 t -> 'a2 t -> 'a3 t **)
+
+  let combine =
+    PTree.combine
+ end
+
+type stateVar =
+| SvT
+| SvX
+| SvXD
+| SvXDD
+| SvCOEFF_OF_REST
+| SvGRAVITY
+| SvT_STOP
+| SvDT
+| SvDT_MAX
+| SvDT_MIN
+| SvDT_PRINT
+
+(** val state_var_eq : stateVar -> stateVar -> bool **)
+
+let state_var_eq r1 r2 =
+  match r1 with
+  | SvT -> (match r2 with
+            | SvT -> true
+            | _ -> false)
+  | SvX -> (match r2 with
+            | SvX -> true
+            | _ -> false)
+  | SvXD -> (match r2 with
+             | SvXD -> true
+             | _ -> false)
+  | SvXDD -> (match r2 with
+              | SvXDD -> true
+              | _ -> false)
+  | SvCOEFF_OF_REST -> (match r2 with
+                        | SvCOEFF_OF_REST -> true
+                        | _ -> false)
+  | SvGRAVITY -> (match r2 with
+                  | SvGRAVITY -> true
+                  | _ -> false)
+  | SvT_STOP -> (match r2 with
+                 | SvT_STOP -> true
+                 | _ -> false)
+  | SvDT -> (match r2 with
+             | SvDT -> true
+             | _ -> false)
+  | SvDT_MAX -> (match r2 with
+                 | SvDT_MAX -> true
+                 | _ -> false)
+  | SvDT_MIN -> (match r2 with
+                 | SvDT_MIN -> true
+                 | _ -> false)
+  | SvDT_PRINT -> (match r2 with
+                   | SvDT_PRINT -> true
+                   | _ -> false)
+
+(** val svIndex : stateVar -> positive **)
+
+let svIndex = function
+| SvT -> XH
+| SvX -> XO XH
+| SvXD -> XI XH
+| SvXDD -> XO (XO XH)
+| SvCOEFF_OF_REST -> XI (XO XH)
+| SvGRAVITY -> XO (XI XH)
+| SvT_STOP -> XI (XI XH)
+| SvDT -> XO (XO (XO XH))
+| SvDT_MAX -> XI (XO (XO XH))
+| SvDT_MIN -> XO (XI (XO XH))
+| SvDT_PRINT -> XI (XI (XO XH))
+
+(** val svStrList : (stateVar * char list) list **)
+
+let svStrList =
+  (SvT, ('T'::[])) :: ((SvX, ('X'::[])) :: ((SvXD, ('X'::('D'::[]))) :: ((SvXDD,
+    ('X'::('D'::('D'::[])))) :: ((SvCOEFF_OF_REST,
+    ('C'::('O'::('E'::('F'::('F'::('_'::('O'::('F'::('_'::('R'::('E'::('S'::('T'::[])))))))))))))) :: ((SvGRAVITY,
+    ('G'::('R'::('A'::('V'::('I'::('T'::('Y'::[])))))))) :: ((SvT_STOP,
+    ('T'::('_'::('S'::('T'::('O'::('P'::[]))))))) :: ((SvDT, ('D'::('T'::[]))) :: ((SvDT_MAX,
+    ('D'::('T'::('_'::('M'::('A'::('X'::[]))))))) :: ((SvDT_MIN,
+    ('D'::('T'::('_'::('M'::('I'::('N'::[]))))))) :: ((SvDT_PRINT,
+    ('D'::('T'::('_'::('P'::('R'::('I'::('N'::('T'::[]))))))))) :: []))))))))))
+
+module SvIndex =
+ struct
+  type t = stateVar
+
+  (** val index : stateVar -> positive **)
+
+  let index =
+    svIndex
+
+  (** val eq : stateVar -> stateVar -> bool **)
+
+  let eq =
+    state_var_eq
+ end
+
+module SvTree = ITree(SvIndex)
+
+type stringSvTreeTy = char list SvTree.t
+
+(** val emptyStringPTree : char list SvTree.t **)
+
+let emptyStringPTree =
+  SvTree.empty
+
+(** val updateStringSvTree : (stateVar * char list) list -> stringSvTreeTy -> stringSvTreeTy **)
+
+let rec updateStringSvTree valList intree =
+  match valList with
+  | [] -> intree
+  | p :: vltail ->
+    let (sv, val0) = p in let tree1 = SvTree.set sv val0 intree in updateStringSvTree vltail tree1
+
+(** val svToStringTree : stringSvTreeTy **)
+
+let svToStringTree =
+  updateStringSvTree svStrList emptyStringPTree
+
+(** val svToStrOpt : stateVar -> char list option **)
+
+let svToStrOpt sv =
+  SvTree.get sv svToStringTree
+
+(** val svToStr : stateVar -> char list **)
+
+let svToStr sv =
+  match svToStrOpt sv with
+  | Some x -> x
+  | None -> []
+
+type floatSvTreeTy = float SvTree.t
+
+(** val emptyFloatPTree : float SvTree.t **)
+
+let emptyFloatPTree =
+  SvTree.empty
+
+(** val updateFloatSvTree : (stateVar * float) list -> floatSvTreeTy -> floatSvTreeTy **)
+
+let rec updateFloatSvTree valList intree =
+  match valList with
+  | [] -> intree
+  | p :: vltail ->
+    let (sv, fval) = p in let tree1 = SvTree.set sv fval intree in updateFloatSvTree vltail tree1
+
+(** val stringKeyValToFloatKeyVal : (stateVar * char list) list -> (stateVar * float) list **)
+
+let rec stringKeyValToFloatKeyVal = function
+| [] -> []
+| p :: tl ->
+  let (sv, str) = p in
+  let tailkvs = stringKeyValToFloatKeyVal tl in
+  (match FloatIO.strToFloat str with
+   | Some fval -> (sv, fval) :: tailkvs
+   | None -> tailkvs)
+
+(** val driver_defaults_str : (stateVar * char list) list **)
+
+let driver_defaults_str =
+  (SvT, ('0'::('.'::('0'::[])))) :: ((SvT_STOP, ('0'::('.'::('0'::[])))) :: ((SvDT,
+    ('0'::('.'::('0'::('0'::('5'::[])))))) :: ((SvDT_MAX,
+    ('0'::('.'::('0'::('0'::('5'::[])))))) :: ((SvDT_MIN,
+    ('0'::('.'::('0'::('0'::('5'::[])))))) :: ((SvDT_PRINT, ('0'::('.'::('0'::('1'::[]))))) :: [])))))
+
+(** val driver_defaults : unit -> (stateVar * float) list **)
+
+let driver_defaults _ =
+  stringKeyValToFloatKeyVal driver_defaults_str
+
+(** val model_default_values_str : (stateVar * char list) list **)
+
+let model_default_values_str =
+  (SvT, ('0'::('.'::('0'::[])))) :: ((SvX, ('1'::('0'::('.'::('0'::[]))))) :: ((SvXD,
+    ('0'::('.'::('0'::[])))) :: ((SvXDD, ('0'::('.'::('0'::[])))) :: ((SvCOEFF_OF_REST,
+    ('0'::('.'::('8'::('0'::[]))))) :: ((SvGRAVITY, ('9'::('.'::('8'::('8'::[]))))) :: ((SvT_STOP,
+    ('1'::('0'::('.'::('0'::[]))))) :: ((SvDT, ('0'::('.'::('0'::('1'::[]))))) :: ((SvDT_MAX,
+    ('0'::('.'::('0'::('0'::('5'::[])))))) :: ((SvDT_MIN,
+    ('0'::('.'::('0'::('0'::('1'::[])))))) :: ((SvDT_PRINT, ('0'::('.'::('0'::('1'::[]))))) :: []))))))))))
+
+(** val model_default_values : unit -> (stateVar * float) list **)
+
+let model_default_values _ =
+  stringKeyValToFloatKeyVal model_default_values_str
+
+(** val state0 : unit -> floatSvTreeTy **)
+
+let state0 _ =
+  let driverState = updateFloatSvTree (driver_defaults ()) emptyFloatPTree in
+  updateFloatSvTree (model_default_values ()) driverState
+
+(** val svGetFloat : stateVar -> floatSvTreeTy -> float **)
+
+let svGetFloat sv tree0 =
+  match SvTree.get sv tree0 with
+  | Some x -> x
+  | None -> Float.zero
+
+(** val modelOutputs : stateVar list **)
+
+let modelOutputs =
+  SvT :: (SvX :: (SvXD :: []))
+
+type flagsTy = { stop_simulation : bool; end_of_run : bool; evaluate_xd : bool }
+
+(** val stop_simulation : flagsTy -> bool **)
+
+let stop_simulation x = x.stop_simulation
+
+(** val end_of_run : flagsTy -> bool **)
+
+let end_of_run x = x.end_of_run
+
+(** val evaluate_xd : flagsTy -> bool **)
+
+let evaluate_xd x = x.evaluate_xd
+
+type eventFuncId =
+| EfiStop
+| EfiAppendSolution
+| EfiTerminateSim
+| EfiFlip_Xd_At_Bounce
+
+type eventTy = { key : char list; time : float; func : eventFuncId }
+
+(** val key : eventTy -> char list **)
+
+let key x = x.key
+
+(** val time : eventTy -> float **)
+
+let time x = x.time
+
+(** val func : eventTy -> eventFuncId **)
+
+let func x = x.func
+
+type logEntryTy = { le_caption : char list; le_vars : (char list * char list) list;
+                    le_events : (char list * char list) list }
+
+type simTy = { vars : floatSvTreeTy; solkeys : stateVar list; solution : char list list list;
+               sim_events : eventTy list; log : logEntryTy list; flags : flagsTy }
+
+(** val vars : simTy -> floatSvTreeTy **)
+
+let vars x = x.vars
+
+(** val solkeys : simTy -> stateVar list **)
+
+let solkeys x = x.solkeys
+
+(** val solution : simTy -> char list list list **)
+
+let solution x = x.solution
+
+(** val sim_events : simTy -> eventTy list **)
+
+let sim_events x = x.sim_events
+
+(** val log : simTy -> logEntryTy list **)
+
+let log x = x.log
+
+(** val flags : simTy -> flagsTy **)
+
+let flags x = x.flags
+
+(** val log_sim : char list -> simTy -> simTy **)
+
+let log_sim _ sim =
+  sim
+
+(** val default_flags : flagsTy **)
+
+let default_flags =
+  { stop_simulation = false; end_of_run = false; evaluate_xd = false }
+
+(** val t_ge_tstop_event_func : eventTy -> simTy -> simTy * float option **)
+
+let t_ge_tstop_event_func _ sim =
+  let sim1 =
+    log_sim
+      ('t'::('_'::('g'::('e'::('_'::('t'::('s'::('t'::('o'::('p'::('_'::('e'::('v'::('e'::('n'::('t'::('_'::('f'::('u'::('n'::('c'::(':'::(' '::('s'::('i'::('m'::('1'::[])))))))))))))))))))))))))))
+      sim
+  in
+  let vars0 = sim1.vars in
+  let t0 = svGetFloat SvT vars0 in
+  let t_stop = svGetFloat SvT_STOP vars0 in
+  let stop_sim = Float.cmp Cge t0 t_stop in
+  let new_flags =
+    set stop_simulation (fun f e -> { stop_simulation = (f e.stop_simulation); end_of_run = e.end_of_run;
+      evaluate_xd = e.evaluate_xd }) (constructor stop_sim) sim1.flags
+  in
+  let result_sim =
+    set flags (fun f e -> { vars = e.vars; solkeys = e.solkeys; solution = e.solution; sim_events =
+      e.sim_events; log = e.log; flags = (f e.flags) }) (constructor new_flags) sim1
+  in
+  let result_log =
+    log_sim
+      ('t'::('_'::('g'::('e'::('_'::('t'::('s'::('t'::('o'::('p'::('_'::('e'::('v'::('e'::('n'::('t'::('_'::('f'::('u'::('n'::('c'::(':'::(' '::('r'::('e'::('s'::('u'::('l'::('t'::('_'::('s'::('i'::('m'::[])))))))))))))))))))))))))))))))))
+      result_sim
+  in
+  (result_log, None)
+
+(** val make_solution_row_helper : floatSvTreeTy -> stateVar list -> char list list **)
+
+let rec make_solution_row_helper vars0 = function
+| [] -> []
+| key0 :: others ->
+  let fval = svGetFloat key0 vars0 in
+  let sval = DebugIO.print_float fval in sval :: (make_solution_row_helper vars0 others)
+
+(** val make_solution_row : simTy -> simTy **)
+
+let make_solution_row sim =
+  let row = make_solution_row_helper sim.vars sim.solkeys in
+  let result_sim =
+    set solution (fun f e -> { vars = e.vars; solkeys = e.solkeys; solution = (f e.solution); sim_events =
+      e.sim_events; log = e.log; flags = e.flags }) (fun old -> row :: old) sim
+  in
+  log_sim
+    ('m'::('a'::('k'::('e'::('_'::('s'::('o'::('l'::('u'::('t'::('i'::('o'::('n'::('_'::('r'::('o'::('w'::(':'::(' '::('r'::('e'::('s'::('u'::('l'::('t'::[])))))))))))))))))))))))))
+    result_sim
+
+(** val append_solution_event_func : eventTy -> simTy -> simTy * float option **)
+
+let append_solution_event_func _ sim =
+  let sim1 = make_solution_row sim in
+  let sim1log =
+    log_sim
+      ('a'::('p'::('p'::('e'::('n'::('d'::('_'::('s'::('o'::('l'::('u'::('t'::('i'::('o'::('n'::('_'::('e'::('v'::('e'::('n'::('t'::('_'::('f'::('u'::('n'::('c'::(':'::('s'::('i'::('m'::('1'::[])))))))))))))))))))))))))))))))
+      sim1
+  in
+  let vars0 = sim1log.vars in
+  let dt_print = svGetFloat SvDT_PRINT vars0 in
+  let t0 = svGetFloat SvT vars0 in let new_t = Float.add t0 dt_print in (sim1log, (Some new_t))
+
+(** val terminate_sim_event_func : eventTy -> simTy -> simTy * float option **)
+
+let terminate_sim_event_func _ sim =
+  let simlog =
+    log_sim
+      ('t'::('e'::('r'::('m'::('i'::('n'::('a'::('t'::('e'::('_'::('s'::('i'::('m'::('_'::('e'::('v'::('e'::('n'::('t'::('_'::('f'::('u'::('n'::('c'::(':'::(' '::('s'::('i'::('m'::[])))))))))))))))))))))))))))))
+      sim
+  in
+  (simlog, None)
+
+(** val driver_default_events : eventTy list **)
+
+let driver_default_events =
+  { key =
+    ('t'::('_'::('g'::('e'::('_'::('t'::('s'::('t'::('o'::('p'::('_'::('e'::('v'::('e'::('n'::('t'::[]))))))))))))))));
+    time = Float.zero; func = EfiStop } :: ({ key =
+    ('a'::('p'::('p'::('e'::('n'::('d'::('_'::('l'::('o'::('g'::('_'::('e'::('v'::('e'::('n'::('t'::[]))))))))))))))));
+    time = Float.zero; func = EfiAppendSolution } :: ({ key =
+    ('t'::('e'::('r'::('m'::('i'::('n'::('a'::('t'::('e'::('_'::('s'::('i'::('m'::('_'::('e'::('v'::('e'::('n'::('t'::[])))))))))))))))))));
+    time = Float.zero; func = EfiTerminateSim } :: []))
+
+(** val default_sim : simTy **)
+
+let default_sim =
+  { vars = (state0 ()); solkeys = modelOutputs; solution = []; sim_events = driver_default_events; log = [];
+    flags = default_flags }
+
+(** val default_sim_log : simTy **)
+
+let default_sim_log =
+  log_sim ('d'::('e'::('f'::('a'::('u'::('l'::('t'::('_'::('s'::('i'::('m'::[]))))))))))) default_sim
+
+(** val f99 : float **)
+
+let f99 =
+  FloatIO.strToFloat' ('9'::('9'::('.'::('0'::[]))))
+
+(** val bounceEvent : eventTy **)
+
+let bounceEvent =
+  { key =
+    ('f'::('l'::('i'::('p'::('_'::('x'::('d'::('_'::('a'::('t'::('_'::('b'::('o'::('u'::('n'::('c'::('e'::('_'::('e'::('v'::('e'::('n'::('t'::[])))))))))))))))))))))));
+    time = f99; func = EfiFlip_Xd_At_Bounce }
+
+(** val init_sim : simTy -> simTy **)
+
+let init_sim sim =
+  let result_sim =
+    set sim_events (fun f e -> { vars = e.vars; solkeys = e.solkeys; solution = e.solution; sim_events =
+      (f e.sim_events); log = e.log; flags = e.flags }) (fun evs -> bounceEvent :: evs) sim
+  in
+  log_sim
+    ('i'::('n'::('i'::('t'::('_'::('s'::('i'::('m'::(':'::(' '::('r'::('e'::('s'::('u'::('l'::('t'::[]))))))))))))))))
+    result_sim
+
+(** val set_vars : simTy -> floatSvTreeTy -> simTy **)
+
+let set_vars sim new_vars =
+  let result_sim =
+    set vars (fun f e -> { vars = (f e.vars); solkeys = e.solkeys; solution = e.solution; sim_events =
+      e.sim_events; log = e.log; flags = e.flags }) (constructor new_vars) sim
+  in
+  log_sim
+    ('s'::('e'::('t'::('_'::('v'::('a'::('r'::('s'::(':'::(' '::('r'::('e'::('s'::('u'::('l'::('t'::[]))))))))))))))))
+    result_sim
+
+(** val flip_xd_at_bounce_event_func : eventTy -> simTy -> simTy * float option **)
+
+let flip_xd_at_bounce_event_func _ sim =
+  let sim' =
+    log_sim
+      ('f'::('l'::('i'::('p'::('_'::('x'::('d'::('_'::('a'::('t'::('_'::('b'::('o'::('u'::('n'::('c'::('e'::('_'::('e'::('v'::('e'::('n'::('t'::('_'::('f'::('u'::('n'::('c'::(':'::(' '::('s'::('i'::('m'::[])))))))))))))))))))))))))))))))))
+      sim
+  in
+  let vars0 = sim'.vars in
+  let coeff_of_rest = svGetFloat SvCOEFF_OF_REST vars0 in
+  let xd = svGetFloat SvXD vars0 in
+  let new_xd = Float.neg (Float.mul coeff_of_rest xd) in
+  let vars' = SvTree.set SvXD new_xd vars0 in
+  let new_flags =
+    set evaluate_xd (fun f e -> { stop_simulation = e.stop_simulation; end_of_run = e.end_of_run;
+      evaluate_xd = (f e.evaluate_xd) }) (constructor true) sim'.flags
+  in
+  let sim2 = set_vars sim' vars' in
+  let result_sim =
+    set flags (fun f e -> { vars = e.vars; solkeys = e.solkeys; solution = e.solution; sim_events =
+      e.sim_events; log = e.log; flags = (f e.flags) }) (constructor new_flags) sim2
+  in
+  let result_log =
+    log_sim
+      ('f'::('l'::('i'::('p'::('_'::('x'::('d'::('_'::('a'::('t'::('_'::('b'::('o'::('u'::('n'::('c'::('e'::('_'::('e'::('v'::('e'::('n'::('t'::('_'::('f'::('u'::('n'::('c'::[]))))))))))))))))))))))))))))
+      result_sim
+  in
+  (result_log, (Some f99))
+
+(** val handle_event : eventTy -> simTy -> simTy * float option **)
+
+let handle_event this sim =
+  let sim_log =
+    log_sim
+      ('h'::('a'::('n'::('d'::('l'::('e'::('_'::('e'::('v'::('e'::('n'::('t'::(':'::('s'::('i'::('m'::[]))))))))))))))))
+      sim
+  in
+  let result =
+    match this.func with
+    | EfiStop -> t_ge_tstop_event_func this sim_log
+    | EfiAppendSolution -> append_solution_event_func this sim_log
+    | EfiTerminateSim -> terminate_sim_event_func this sim_log
+    | EfiFlip_Xd_At_Bounce -> flip_xd_at_bounce_event_func this sim_log
+  in
+  let (result_sim, maybefloat) = result in
+  let result_log =
+    log_sim
+      ('h'::('a'::('n'::('d'::('l'::('e'::('_'::('e'::('v'::('e'::('n'::('t'::(':'::('r'::('e'::('s'::('u'::('l'::('t'::[])))))))))))))))))))
+      result_sim
+  in
+  (result_log, maybefloat)
+
+(** val set_var : stateVar -> float -> simTy -> simTy **)
+
+let set_var key0 val0 sim =
+  let sim_log = log_sim ('s'::('e'::('t'::('_'::('v'::('a'::('r'::(':'::('s'::('i'::('m'::[]))))))))))) sim in
+  let result_sim =
+    set vars (fun f e -> { vars = (f e.vars); solkeys = e.solkeys; solution = e.solution; sim_events =
+      e.sim_events; log = e.log; flags = e.flags }) (constructor (SvTree.set key0 val0 sim.vars)) sim_log
+  in
+  log_sim
+    ('s'::('e'::('t'::('_'::('v'::('a'::('r'::(':'::('r'::('e'::('s'::('u'::('l'::('t'::[]))))))))))))))
+    result_sim
+
+(** val fhalf : float **)
+
+let fhalf =
+  FloatIO.strToFloat' ('0'::('.'::('5'::[])))
+
+(** val ftwo : float **)
+
+let ftwo =
+  FloatIO.strToFloat' ('2'::('.'::('0'::[])))
+
+(** val epsilon : float **)
+
+let epsilon =
+  FloatIO.strToFloat' ('0'::('.'::('0'::('0'::('0'::('0'::('0'::('0'::('0'::('0'::('0'::('1'::[]))))))))))))
+
+(** val efi_eqb : eventFuncId -> eventFuncId -> bool **)
+
+let efi_eqb fi1 fi2 =
+  match fi1 with
+  | EfiStop -> (match fi2 with
+                | EfiStop -> true
+                | _ -> false)
+  | EfiAppendSolution -> (match fi2 with
+                          | EfiAppendSolution -> true
+                          | _ -> false)
+  | EfiTerminateSim -> (match fi2 with
+                        | EfiTerminateSim -> true
+                        | _ -> false)
+  | EfiFlip_Xd_At_Bounce -> (match fi2 with
+                             | EfiFlip_Xd_At_Bounce -> true
+                             | _ -> false)
+
+(** val schedule_event : eventTy list -> eventFuncId -> float -> eventTy list **)
+
+let rec schedule_event evs efi new_time =
+  match evs with
+  | [] -> []
+  | ev :: evtl ->
+    let ev' =
+      if efi_eqb ev.func efi
+      then set time (fun f e -> { key = e.key; time = (f e.time); func = e.func }) (constructor new_time) ev
+      else ev
+    in
+    ev' :: (schedule_event evtl efi new_time)
+
+(** val sqrt : float -> float **)
+
+let sqrt arg =
+  b64_sqrt Mode_NE arg
+
+(** val fone : float **)
+
+let fone =
+  FloatIO.strToFloat' ('1'::('.'::('0'::[])))
+
+(** val differential_equations : simTy -> simTy **)
+
+let differential_equations sim =
+  let sim_log =
+    log_sim
+      ('d'::('i'::('f'::('f'::('e'::('r'::('e'::('n'::('t'::('i'::('a'::('l'::('_'::('e'::('q'::('u'::('a'::('t'::('i'::('o'::('n'::('s'::[]))))))))))))))))))))))
+      sim
+  in
+  let vars0 = sim_log.vars in
+  let t0 = svGetFloat SvT vars0 in
+  let x = svGetFloat SvX vars0 in
+  let xd = svGetFloat SvXD vars0 in
+  let dt_min = svGetFloat SvDT_MIN vars0 in
+  let dt_max = svGetFloat SvDT_MAX vars0 in
+  let gravity = svGetFloat SvGRAVITY vars0 in
+  let t_stop = svGetFloat SvT_STOP vars0 in
+  let xdd = Float.neg gravity in
+  let sim1 = set_var SvXDD xdd sim_log in
+  let sim1log =
+    log_sim
+      ('d'::('i'::('f'::('f'::('e'::('r'::('e'::('n'::('t'::('i'::('a'::('l'::('_'::('e'::('q'::('u'::('a'::('t'::('i'::('o'::('n'::('s'::(':'::('s'::('i'::('m'::('1'::[])))))))))))))))))))))))))))
+      sim1
+  in
+  let est_max =
+    Float.add (Float.add x (Float.mul xd dt_max)) (Float.mul (Float.mul (Float.mul fhalf xdd) dt_max) dt_max)
+  in
+  let dt_impact = Float.add t_stop fone in
+  let dt_impact2 =
+    if Float.cmp Cle est_max Float.zero
+    then let est_min =
+           Float.add (Float.add x (Float.mul xd dt_min))
+             (Float.mul (Float.mul (Float.mul fhalf xdd) dt_min) dt_min)
+         in
+         if Float.cmp Cle est_min Float.zero
+         then Float.zero
+         else let dt_impact3 =
+                Float.div
+                  (Float.sub (Float.neg xd)
+                    (sqrt (Float.sub (Float.mul xd xd) (Float.mul (Float.mul ftwo x) xdd))))
+                  (Float.mul ftwo x)
+              in
+              if Float.cmp Cgt (Float.sub dt_min dt_impact3) epsilon
+              then Float.div
+                     (Float.add (Float.neg xd)
+                       (sqrt (Float.sub (Float.mul xd xd) (Float.mul (Float.mul ftwo x) xdd))))
+                     (Float.mul ftwo x)
+              else dt_impact3
+    else dt_impact
+  in
+  let impact_time = Float.add t0 dt_impact2 in
+  let events' = schedule_event sim1log.sim_events EfiFlip_Xd_At_Bounce impact_time in
+  let result_sim =
+    set sim_events (fun f e -> { vars = e.vars; solkeys = e.solkeys; solution = e.solution; sim_events =
+      (f e.sim_events); log = e.log; flags = e.flags }) (constructor events') sim1log
+  in
+  log_sim
+    ('d'::('i'::('f'::('f'::('e'::('r'::('e'::('n'::('t'::('i'::('a'::('l'::('_'::('e'::('q'::('u'::('a'::('t'::('i'::('o'::('n'::('s'::[]))))))))))))))))))))))
+    result_sim
+
+(** val zofFloat : float -> z **)
+
+let zofFloat f =
+  match zofB (Zpos (XI (XO (XI (XO (XI XH)))))) (Zpos (XO (XO (XO (XO (XO (XO (XO (XO (XO (XO XH))))))))))) f with
+  | Some z0 -> z0
+  | None -> Z0
+
+(** val round : float -> float **)
+
+let round f =
+  let z0 = zofFloat f in FloatIO.coq_Z_to_float z0
+
+(** val tenTo6 : float **)
+
+let tenTo6 =
+  FloatIO.strToFloat' ('1'::('.'::('e'::('6'::[]))))
+
+(** val process_one_event : eventTy -> simTy -> eventTy * simTy **)
+
+let process_one_event ev sim =
+  let sim_log =
+    log_sim
+      ('p'::('r'::('o'::('c'::('e'::('s'::('s'::('_'::('o'::('n'::('e'::('_'::('e'::('v'::('e'::('n'::('t'::(':'::('s'::('i'::('m'::[])))))))))))))))))))))
+      sim
+  in
+  let vars0 = sim_log.vars in
+  let t0 = svGetFloat SvT vars0 in
+  let dt_min = svGetFloat SvDT_MIN vars0 in
+  let et = ev.time in
+  let etdelta = round (Float.mul (Float.sub et t0) tenTo6) in
+  let minrnd = round (Float.mul dt_min tenTo6) in
+  let (ev', result_sim) =
+    if Float.cmp Clt etdelta minrnd
+    then let (sim2, new_time_opt) = handle_event ev sim_log in
+         let sim2log =
+           log_sim
+             ('p'::('r'::('o'::('c'::('e'::('s'::('s'::('_'::('o'::('n'::('e'::('_'::('e'::('v'::('e'::('n'::('t'::(':'::('s'::('i'::('m'::('2'::[]))))))))))))))))))))))
+             sim2
+         in
+         (match new_time_opt with
+          | Some new_time ->
+            ((set time (fun f e -> { key = e.key; time = (f e.time); func = e.func }) (constructor new_time)
+               ev), sim2log)
+          | None -> (ev, sim2log))
+    else (ev, sim_log)
+  in
+  let result_log =
+    log_sim
+      ('p'::('r'::('o'::('c'::('e'::('s'::('s'::('_'::('o'::('n'::('e'::('_'::('e'::('v'::('e'::('n'::('t'::[])))))))))))))))))
+      result_sim
+  in
+  (ev', result_log)
+
+(** val process_events_helper : eventTy list -> simTy -> eventTy list * simTy **)
+
+let rec process_events_helper evs sim =
+  match evs with
+  | [] -> ([], sim)
+  | ev :: evtl ->
+    let (ev', sim') = process_one_event ev sim in
+    let (evs', sim'') = process_events_helper evtl sim' in ((ev' :: evs'), sim'')
+
+(** val min_event_time : eventTy list -> float -> float **)
+
+let rec min_event_time evs min_so_far =
+  match evs with
+  | [] -> min_so_far
+  | ev :: evtl ->
+    let et = ev.time in
+    let new_min = if (&&) (Float.cmp Cgt et Float.zero) (Float.cmp Clt et min_so_far) then et else min_so_far
+    in
+    min_event_time evtl new_min
+
+(** val process_events : simTy -> simTy **)
+
+let process_events sim =
+  let sim_log =
+    log_sim
+      ('p'::('r'::('o'::('c'::('e'::('s'::('s'::('_'::('e'::('v'::('e'::('n'::('t'::('s'::(':'::('s'::('i'::('m'::[]))))))))))))))))))
+      sim
+  in
+  let vars0 = sim_log.vars in
+  let events = sim_log.sim_events in
+  let result_sim =
+    match events with
+    | [] -> set_var SvDT (svGetFloat SvDT_MAX vars0) sim_log
+    | _ :: _ ->
+      let t0 = svGetFloat SvT vars0 in
+      let dt_max = svGetFloat SvDT_MAX vars0 in
+      let (evs', sim1) = process_events_helper events sim_log in
+      let sim1log =
+        log_sim
+          ('p'::('r'::('o'::('c'::('e'::('s'::('s'::('_'::('e'::('v'::('e'::('n'::('t'::('s'::(':'::('s'::('i'::('m'::('1'::[])))))))))))))))))))
+          sim1
+      in
+      let vars' = sim1log.vars in
+      let min_time0 = svGetFloat SvT_STOP vars' in
+      let min_time = min_event_time evs' min_time0 in
+      let time_to_next_event = Float.sub min_time t0 in
+      let new_dt =
+        if (&&) (Float.cmp Cgt time_to_next_event Float.zero)
+             (Float.cmp Cgt (Float.sub dt_max time_to_next_event) epsilon)
+        then time_to_next_event
+        else dt_max
+      in
+      let sim3 = set_var SvDT new_dt sim1log in
+      let sim4 =
+        set sim_events (fun f e -> { vars = e.vars; solkeys = e.solkeys; solution = e.solution; sim_events =
+          (f e.sim_events); log = e.log; flags = e.flags }) (constructor evs') sim3
+      in
+      log_sim
+        ('p'::('r'::('o'::('c'::('e'::('s'::('s'::('_'::('e'::('v'::('e'::('n'::('t'::('s'::(':'::('s'::('i'::('m'::('4'::[])))))))))))))))))))
+        sim4
+  in
+  log_sim
+    ('p'::('r'::('o'::('c'::('e'::('s'::('s'::('_'::('e'::('v'::('e'::('n'::('t'::('s'::(':'::('r'::('e'::('s'::('u'::('l'::('t'::[])))))))))))))))))))))
+    result_sim
+
+(** val advance_states : (stateVar * stateVar) list -> float -> simTy -> simTy **)
+
+let rec advance_states pairs dt sim =
+  let result_sim =
+    match pairs with
+    | [] -> sim
+    | p :: pairstl ->
+      let (sv, svd) = p in
+      let vars0 = sim.vars in
+      let el = svGetFloat sv vars0 in
+      let eld = svGetFloat svd vars0 in
+      let el' = Float.add el (Float.mul eld dt) in
+      let sim1 = set_var sv el' sim in
+      let sim1log =
+        log_sim
+          ('a'::('d'::('v'::('a'::('n'::('c'::('e'::('_'::('s'::('t'::('a'::('t'::('e'::('s'::(':'::('s'::('i'::('m'::('1'::[])))))))))))))))))))
+          sim1
+      in
+      advance_states pairstl dt sim1log
+  in
+  log_sim
+    ('a'::('d'::('v'::('a'::('n'::('c'::('e'::('_'::('s'::('t'::('a'::('t'::('e'::('s'::(':'::('r'::('e'::('s'::('u'::('l'::('t'::[])))))))))))))))))))))
+    result_sim
+
+(** val advance_model : simTy -> simTy **)
+
+let advance_model sim =
+  let sim_log =
+    log_sim
+      ('a'::('d'::('v'::('a'::('n'::('c'::('e'::('_'::('m'::('o'::('d'::('e'::('l'::(':'::('s'::('i'::('m'::[])))))))))))))))))
+      sim
+  in
+  let vars0 = sim_log.vars in
+  let dt = svGetFloat SvDT vars0 in
+  let pairs = (SvX, SvXD) :: ((SvXD, SvXDD) :: []) in
+  let sim2 = advance_states pairs dt sim_log in
+  let sim2log =
+    log_sim
+      ('a'::('d'::('v'::('a'::('n'::('c'::('e'::('_'::('m'::('o'::('d'::('e'::('l'::(':'::('s'::('i'::('m'::('2'::[]))))))))))))))))))
+      sim2
+  in
+  let vars' = sim2log.vars in
+  let t0 = svGetFloat SvT vars' in
+  let new_t = Float.add t0 dt in
+  let rounded_new_t = Float.div (round (Float.mul new_t tenTo6)) tenTo6 in
+  let result_sim = set_var SvT rounded_new_t sim2log in
+  log_sim
+    ('a'::('d'::('v'::('a'::('n'::('c'::('e'::('_'::('m'::('o'::('d'::('e'::('l'::(':'::('r'::('e'::('s'::('u'::('l'::('t'::[]))))))))))))))))))))
+    result_sim
+
+(** val oneStep : simTy -> simTy **)
+
+let oneStep sim =
+  let sim_log = log_sim ('o'::('n'::('e'::('S'::('t'::('e'::('p'::(':'::('s'::('i'::('m'::[]))))))))))) sim in
+  let sim1 = differential_equations sim_log in
+  let sim1log =
+    log_sim ('o'::('n'::('e'::('S'::('t'::('e'::('p'::(':'::('s'::('i'::('m'::('1'::[])))))))))))) sim1
+  in
+  let sim2 = process_events sim1log in
+  let sim2log =
+    log_sim ('o'::('n'::('e'::('S'::('t'::('e'::('p'::(':'::('s'::('i'::('m'::('2'::[])))))))))))) sim2
+  in
+  let sim3 =
+    if sim2log.flags.evaluate_xd
+    then let sim4 = differential_equations sim2log in
+         let sim4log =
+           log_sim ('o'::('n'::('e'::('S'::('t'::('e'::('p'::(':'::('s'::('i'::('m'::('4'::[])))))))))))) sim4
+         in
+         let flags4 = sim4log.flags in
+         let flags4' =
+           set evaluate_xd (fun f e -> { stop_simulation = e.stop_simulation; end_of_run = e.end_of_run;
+             evaluate_xd = (f e.evaluate_xd) }) (constructor false) flags4
+         in
+         let sim6 =
+           set flags (fun f e -> { vars = e.vars; solkeys = e.solkeys; solution = e.solution; sim_events =
+             e.sim_events; log = e.log; flags = (f e.flags) }) (constructor flags4') sim4log
+         in
+         log_sim ('o'::('n'::('e'::('S'::('t'::('e'::('p'::(':'::('s'::('i'::('m'::('6'::[])))))))))))) sim6
+    else sim2log
+  in
+  let sim3log =
+    log_sim ('o'::('n'::('e'::('S'::('t'::('e'::('p'::(':'::('s'::('i'::('m'::('3'::[])))))))))))) sim3
+  in
+  let sim5 = advance_model sim3log in
+  log_sim ('o'::('n'::('e'::('S'::('t'::('e'::('p'::(':'::('s'::('i'::('m'::('5'::[])))))))))))) sim5
+
+(** val run_sim_loop : z -> simTy -> simTy **)
+
+let rec run_sim_loop steps sim =
+  if zle Z0 steps
+  then if (||) sim.flags.end_of_run sim.flags.stop_simulation
+       then sim
+       else run_sim_loop (Z.sub steps (Zpos XH)) (oneStep sim)
+  else sim
+
+(** val run_sim : simTy -> simTy **)
+
+let run_sim sim =
+  let sim_log = log_sim ('r'::('u'::('n'::('_'::('s'::('i'::('m'::(':'::('s'::('i'::('m'::[]))))))))))) sim in
+  let vars0 = sim_log.vars in
+  let dtmin = svGetFloat SvDT_MIN vars0 in
+  let tstop = svGetFloat SvT_STOP vars0 in
+  let max_steps_float = Float.div tstop dtmin in
+  let steps = zofFloat max_steps_float in
+  let result_sim = run_sim_loop steps sim_log in
+  log_sim
+    ('r'::('u'::('n'::('_'::('s'::('i'::('m'::(':'::('r'::('e'::('s'::('u'::('l'::('t'::[]))))))))))))))
+    result_sim
+
+(** val sim_in : unit -> simTy **)
+
+let sim_in _ =
+  let sim1log =
+    log_sim ('s'::('i'::('m'::('_'::('i'::('n'::(':'::('s'::('i'::('m'::('1'::[]))))))))))) default_sim_log
+  in
+  let sim2 = init_sim sim1log in
+  let sim2log = log_sim ('s'::('i'::('m'::('_'::('i'::('n'::(':'::('s'::('i'::('m'::('2'::[]))))))))))) sim2
+  in
+  let sim3 = set_var SvCOEFF_OF_REST (FloatIO.strToFloat' ('0'::('.'::('8'::('8'::[]))))) sim2log in
+  let sim3log = log_sim ('s'::('i'::('m'::('_'::('i'::('n'::(':'::('s'::('i'::('m'::('3'::[]))))))))))) sim3
+  in
+  let sim4 = set_var SvGRAVITY (FloatIO.strToFloat' ('9'::('.'::('8'::('8'::[]))))) sim3log in
+  log_sim ('s'::('i'::('m'::('_'::('i'::('n'::(':'::('s'::('i'::('m'::('4'::[]))))))))))) sim4
+
+(** val main : unit -> simTy **)
+
+let main _ =
+  let sim1 = sim_in () in
+  let sim2 = run_sim sim1 in
+  let sim2log =
+    log_sim
+      ('s'::('i'::('m'::('_'::('m'::('a'::('i'::('n'::(':'::('r'::('e'::('s'::('u'::('l'::('t'::[])))))))))))))))
+      sim2
+  in
+  let sim3 =
+    set solution (fun f e -> { vars = e.vars; solkeys = e.solkeys; solution = (f e.solution); sim_events =
+      e.sim_events; log = e.log; flags = e.flags }) rev sim2log
+  in
+  set log (fun f e -> { vars = e.vars; solkeys = e.solkeys; solution = e.solution; sim_events = e.sim_events;
+    log = (f e.log); flags = e.flags }) rev sim3
