formal/coqimp/extraction/Top.mli
@@ -1,0 +1,839 @@
+
+type __ = Obj.t
+
+val xorb : bool -> bool -> bool
+
+val negb : bool -> bool
+
+type nat =
+| O
+| S of nat
+
+val app : 'a1 list -> 'a1 list -> 'a1 list
+
+type comparison =
+| Eq
+| Lt
+| Gt
+
+val compOpp : comparison -> comparison
+
+type 'a sig0 = 'a
+  (* singleton inductive, whose constructor was exist *)
+
+
+
+type uint =
+| Nil
+| D0 of uint
+| D1 of uint
+| D2 of uint
+| D3 of uint
+| D4 of uint
+| D5 of uint
+| D6 of uint
+| D7 of uint
+| D8 of uint
+| D9 of uint
+
+type int =
+| Pos of uint
+| Neg of uint
+
+val nzhead : uint -> uint
+
+val unorm : uint -> uint
+
+val norm : int -> int
+
+val pred : nat -> nat
+
+val sub : nat -> nat -> nat
+
+type ('e, 't) reader = 'e -> 't
+
+val constructor : 'a2 -> ('a1, 'a2) reader
+
+type ('r, 't) setter = ('t -> 't) -> 'r -> 'r
+  (* singleton inductive, whose constructor was Build_Setter *)
+
+val set : ('a1 -> 'a2) -> ('a1, 'a2) setter -> ('a2 -> 'a2) -> 'a1 -> 'a1
+
+val eqb : bool -> bool -> bool
+
+module Nat :
+ sig
+  val leb : nat -> nat -> bool
+
+  val ltb : nat -> nat -> bool
+ end
+
+type positive =
+| XI of positive
+| XO of positive
+| XH
+
+type n =
+| N0
+| Npos of positive
+
+type z =
+| Z0
+| Zpos of positive
+| Zneg of positive
+
+module Pos :
+ sig
+  type mask =
+  | IsNul
+  | IsPos of positive
+  | IsNeg
+ end
+
+module Coq_Pos :
+ sig
+  val succ : positive -> positive
+
+  val add : positive -> positive -> positive
+
+  val add_carry : positive -> positive -> positive
+
+  val pred_double : positive -> positive
+
+  type mask = Pos.mask =
+  | IsNul
+  | IsPos of positive
+  | IsNeg
+
+  val succ_double_mask : mask -> mask
+
+  val double_mask : mask -> mask
+
+  val double_pred_mask : positive -> mask
+
+  val sub_mask : positive -> positive -> mask
+
+  val sub_mask_carry : positive -> positive -> mask
+
+  val mul : positive -> positive -> positive
+
+  val iter : ('a1 -> 'a1) -> 'a1 -> positive -> 'a1
+
+  val square : positive -> positive
+
+  val div2 : positive -> positive
+
+  val div2_up : positive -> positive
+
+  val size : positive -> positive
+
+  val compare_cont : comparison -> positive -> positive -> comparison
+
+  val compare : positive -> positive -> comparison
+
+  val eqb : positive -> positive -> bool
+
+  val leb : positive -> positive -> bool
+
+  val sqrtrem_step : (positive -> positive) -> (positive -> positive) -> (positive * mask) -> positive * mask
+
+  val sqrtrem : positive -> positive * mask
+
+  val coq_lor : positive -> positive -> positive
+
+  val of_succ_nat : nat -> positive
+
+  val of_uint_acc : uint -> positive -> positive
+
+  val of_uint : uint -> n
+
+  val eq_dec : positive -> positive -> bool
+ end
+
+val rev : 'a1 list -> 'a1 list
+
+module Z :
+ sig
+  val double : z -> z
+
+  val succ_double : z -> z
+
+  val pred_double : z -> z
+
+  val pos_sub : positive -> positive -> z
+
+  val add : z -> z -> z
+
+  val opp : z -> z
+
+  val succ : z -> z
+
+  val pred : z -> z
+
+  val sub : z -> z -> z
+
+  val mul : z -> z -> z
+
+  val pow_pos : z -> positive -> z
+
+  val pow : z -> z -> z
+
+  val compare : z -> z -> comparison
+
+  val leb : z -> z -> bool
+
+  val ltb : z -> z -> bool
+
+  val eqb : z -> z -> bool
+
+  val max : z -> z -> z
+
+  val min : z -> z -> z
+
+  val of_nat : nat -> z
+
+  val of_N : n -> z
+
+  val of_uint : uint -> z
+
+  val of_int : int -> z
+
+  val pos_div_eucl : positive -> z -> z * z
+
+  val div_eucl : z -> z -> z * z
+
+  val div : z -> z -> z
+
+  val modulo : z -> z -> z
+
+  val div2 : z -> z
+
+  val log2 : z -> z
+
+  val sqrtrem : z -> z * z
+
+  val shiftl : z -> z -> z
+
+  val eq_dec : z -> z -> bool
+
+  val log2_up : z -> z
+ end
+
+val z_lt_dec : z -> z -> bool
+
+val z_le_dec : z -> z -> bool
+
+val z_le_gt_dec : z -> z -> bool
+
+val zeq_bool : z -> z -> bool
+
+val append : char list -> char list -> char list
+
+val length : char list -> nat
+
+val substring : nat -> nat -> char list -> char list
+
+val prefix : char list -> char list -> bool
+
+val index : nat -> char list -> char list -> nat option
+
+val shift_nat : nat -> positive -> positive
+
+val shift_pos : positive -> positive -> positive
+
+val two_power_nat : nat -> z
+
+val zeq : z -> z -> bool
+
+val zlt : z -> z -> bool
+
+val zle : z -> z -> bool
+
+val option_map : ('a1 -> 'a2) -> 'a1 option -> 'a2 option
+
+val zeven : z -> bool
+
+type radix = z
+  (* singleton inductive, whose constructor was Build_radix *)
+
+val radix_val : radix -> z
+
+val radix2 : radix
+
+val cond_Zopp : bool -> z -> z
+
+val zpos_div_eucl_aux1 : positive -> positive -> z * z
+
+val zpos_div_eucl_aux : positive -> positive -> z * z
+
+val zfast_div_eucl : z -> z -> z * z
+
+val iter_nat : ('a1 -> 'a1) -> nat -> 'a1 -> 'a1
+
+val iter_pos : ('a1 -> 'a1) -> positive -> 'a1 -> 'a1
+
+val fLT_exp : z -> z -> z -> z
+
+val digits2_pos : positive -> positive
+
+val zdigits2 : z -> z
+
+type location =
+| Loc_Exact
+| Loc_Inexact of comparison
+
+val new_location_even : z -> z -> location -> location
+
+val new_location_odd : z -> z -> location -> location
+
+val new_location : z -> z -> location -> location
+
+val cond_incr : bool -> z -> z
+
+val round_sign_DN : bool -> location -> bool
+
+val round_sign_UP : bool -> location -> bool
+
+val round_N : bool -> location -> bool
+
+type full_float =
+| F754_zero of bool
+| F754_infinity of bool
+| F754_nan of bool * positive
+| F754_finite of bool * positive * z
+
+type nan_pl = positive
+
+type binary_float =
+| B754_zero of bool
+| B754_infinity of bool
+| B754_nan of bool * nan_pl
+| B754_finite of bool * positive * z
+
+val fF2B : z -> z -> full_float -> binary_float
+
+val bopp : z -> z -> (bool -> nan_pl -> bool * nan_pl) -> binary_float -> binary_float
+
+val babs : z -> z -> (bool -> nan_pl -> bool * nan_pl) -> binary_float -> binary_float
+
+val bcompare : z -> z -> binary_float -> binary_float -> comparison option
+
+type shr_record = { shr_m : z; shr_r : bool; shr_s : bool }
+
+val shr_m : shr_record -> z
+
+val shr_1 : shr_record -> shr_record
+
+val loc_of_shr_record : shr_record -> location
+
+val shr_record_of_loc : z -> location -> shr_record
+
+val shr : shr_record -> z -> z -> shr_record * z
+
+val shr_fexp : z -> z -> z -> z -> location -> shr_record * z
+
+type mode =
+| Mode_NE
+| Mode_ZR
+| Mode_DN
+| Mode_UP
+| Mode_NA
+
+val choice_mode : mode -> bool -> z -> location -> z
+
+val overflow_to_inf : mode -> bool -> bool
+
+val binary_overflow : z -> z -> mode -> bool -> full_float
+
+val binary_round_aux : z -> z -> mode -> bool -> positive -> z -> location -> full_float
+
+val bmult :
+  z -> z -> (binary_float -> binary_float -> bool * nan_pl) -> mode -> binary_float -> binary_float ->
+  binary_float
+
+val shl_align : positive -> z -> z -> positive * z
+
+val shl_align_fexp : z -> z -> positive -> z -> positive * z
+
+val binary_round : z -> z -> mode -> bool -> positive -> z -> full_float
+
+val binary_normalize : z -> z -> mode -> z -> z -> bool -> binary_float
+
+val bplus :
+  z -> z -> (binary_float -> binary_float -> bool * nan_pl) -> mode -> binary_float -> binary_float ->
+  binary_float
+
+val bminus :
+  z -> z -> (binary_float -> binary_float -> bool * nan_pl) -> mode -> binary_float -> binary_float ->
+  binary_float
+
+val fdiv_core_binary : z -> z -> z -> z -> z -> (z * z) * location
+
+val bdiv :
+  z -> z -> (binary_float -> binary_float -> bool * nan_pl) -> mode -> binary_float -> binary_float ->
+  binary_float
+
+val fsqrt_core_binary : z -> z -> z -> (z * z) * location
+
+val bsqrt : z -> z -> (binary_float -> bool * nan_pl) -> mode -> binary_float -> binary_float
+
+type binary64 = binary_float
+
+val default_nan_pl64 : bool * nan_pl
+
+val unop_nan_pl64 : binary64 -> bool * nan_pl
+
+val b64_sqrt : mode -> binary_float -> binary_float
+
+val default_pl_64 : bool * nan_pl
+
+val choose_binop_pl_64 : bool -> nan_pl -> bool -> nan_pl -> bool
+
+type comparison0 =
+| Ceq
+| Cne
+| Clt
+| Cle
+| Cgt
+| Cge
+
+module Wordsize_64 :
+ sig
+  val wordsize : nat
+ end
+
+module Int64 :
+ sig
+  val wordsize : nat
+
+  val modulus : z
+
+  val half_modulus : z
+
+  val max_signed : z
+
+  val min_signed : z
+
+  type int = z
+    (* singleton inductive, whose constructor was mkint *)
+
+  val intval : int -> z
+
+  val coq_P_mod_two_p : positive -> nat -> z
+
+  val coq_Z_mod_modulus : z -> z
+
+  val unsigned : int -> z
+
+  val signed : int -> z
+
+  val repr : z -> int
+ end
+
+val bofZ : z -> z -> z -> binary_float
+
+val zofB : z -> z -> binary_float -> z option
+
+val zofB_range : z -> z -> binary_float -> z -> z -> z option
+
+val pos_pow : positive -> positive -> positive
+
+val bparse : z -> z -> positive -> positive -> z -> binary_float
+
+type float = binary64
+
+val cmp_of_comparison : comparison0 -> comparison option -> bool
+
+module Float :
+ sig
+  val transform_quiet_pl : nan_pl -> nan_pl
+
+  val neg_pl : bool -> nan_pl -> bool * nan_pl
+
+  val abs_pl : bool -> nan_pl -> bool * nan_pl
+
+  val binop_pl : binary64 -> binary64 -> bool * nan_pl
+
+  val zero : float
+
+  val neg : float -> float
+
+  val abs : float -> float
+
+  val add : float -> float -> float
+
+  val sub : float -> float -> float
+
+  val mul : float -> float -> float
+
+  val div : float -> float -> float
+
+  val compare : float -> float -> comparison option
+
+  val cmp : comparison0 -> float -> float -> bool
+
+  val to_long : float -> Int64.int option
+
+  val from_parsed : positive -> positive -> z -> float
+ end
+
+type 'm monadOps = { bind : (__ -> __ -> 'm -> (__ -> 'm) -> 'm); ret : (__ -> __ -> 'm) }
+
+val bind : 'a1 monadOps -> 'a1 -> ('a2 -> 'a1) -> 'a1
+
+val ret : 'a1 monadOps -> 'a2 -> 'a1
+
+type 't monadTransformerOps = { tops : (__ -> __ monadOps -> 't monadOps);
+                                lift : (__ -> __ monadOps -> __ -> __ -> 't) }
+
+val tops : 'a1 monadTransformerOps -> 'a2 monadOps -> 'a1 monadOps
+
+val idM : __ monadOps
+
+val monad_of_transformer : 'a1 monadTransformerOps -> 'a1 monadOps
+
+val optionT : __ monadTransformerOps
+
+val optionM : __ option monadOps
+
+module FloatIO :
+ sig
+  val coq_Z_to_float : z -> float
+
+  module Details :
+   sig
+    val precision_of_float : z
+
+    val log10of2scaled3 : z
+
+    val strToUintHelper : char list -> uint option
+
+    val strToUint : char list -> uint option
+
+    val strToIntHelper : char list -> int option
+
+    val strToInt : char list -> int option
+
+    val strToZ : char list -> z option
+
+    val splitAtExponent : char list -> char list * char list
+
+    val splitAtPoint : char list -> char list * char list
+
+    val decomposeFloatString : char list -> (char list * char list) * char list
+
+    val strToFloatHelper : char list -> (z * z) option
+
+    val strToFloat : char list -> float option
+
+    val scale_exp : z -> z -> z
+
+    val digits : z -> char list
+
+    val repeat_string : nat -> char list -> char list
+
+    val coq_Z_to_string_base10_aux : nat -> nat -> z -> char list
+
+    val coq_Z_to_string_base10 : nat -> z -> char list
+
+    val scaled_float_to_Z : float -> z -> z
+
+    val insert_decimal : char list -> nat -> char list
+
+    val float_to_string_unsigned : float -> nat -> char list
+
+    val float_to_string_unpadded : float -> nat -> char list
+
+    val pad_to_width : nat -> char list -> char list
+
+    val float_to_string : nat -> nat -> float -> char list
+   end
+
+  val coq_Z_to_string_base10 : nat -> z -> char list
+
+  val float_to_string : nat -> nat -> float -> char list
+
+  val strToFloat : char list -> float option
+
+  val strToFloat' : char list -> float
+ end
+
+module DebugIO :
+ sig
+  val width : nat
+
+  val fdigs : nat
+
+  val print_float : float -> char list
+
+  val print_Z : z -> char list
+ end
+
+module PTree :
+ sig
+  type 'a tree =
+  | Leaf
+  | Node of 'a tree * 'a option * 'a tree
+
+  type 'a t = 'a tree
+
+  val empty : 'a1 t
+
+  val get : positive -> 'a1 t -> 'a1 option
+
+  val set : positive -> 'a1 -> 'a1 t -> 'a1 t
+
+  val remove : positive -> 'a1 t -> 'a1 t
+
+  val bempty : 'a1 t -> bool
+
+  val beq : ('a1 -> 'a1 -> bool) -> 'a1 t -> 'a1 t -> bool
+
+  val prev_append : positive -> positive -> positive
+
+  val prev : positive -> positive
+
+  val coq_Node' : 'a1 t -> 'a1 option -> 'a1 t -> 'a1 t
+
+  val xcombine_l : ('a1 option -> 'a2 option -> 'a3 option) -> 'a1 t -> 'a3 t
+
+  val xcombine_r : ('a1 option -> 'a2 option -> 'a3 option) -> 'a2 t -> 'a3 t
+
+  val combine : ('a1 option -> 'a2 option -> 'a3 option) -> 'a1 t -> 'a2 t -> 'a3 t
+
+  val xelements : 'a1 t -> positive -> (positive * 'a1) list -> (positive * 'a1) list
+
+  val elements : 'a1 t -> (positive * 'a1) list
+ end
+
+module type INDEXED_TYPE =
+ sig
+  type t
+
+  val index : t -> positive
+
+  val eq : t -> t -> bool
+ end
+
+module ITree :
+ functor (X:INDEXED_TYPE) ->
+ sig
+  type elt = X.t
+
+  val elt_eq : X.t -> X.t -> bool
+
+  type 'x t = 'x PTree.t
+
+  val empty : 'a1 t
+
+  val get : elt -> 'a1 t -> 'a1 option
+
+  val set : elt -> 'a1 -> 'a1 t -> 'a1 t
+
+  val remove : elt -> 'a1 t -> 'a1 t
+
+  val beq : ('a1 -> 'a1 -> bool) -> 'a1 t -> 'a1 t -> bool
+
+  val combine : ('a1 option -> 'a2 option -> 'a3 option) -> 'a1 t -> 'a2 t -> 'a3 t
+ end
+
+type stateVar =
+| SvT
+| SvX
+| SvXD
+| SvXDD
+| SvCOEFF_OF_REST
+| SvGRAVITY
+| SvT_STOP
+| SvDT
+| SvDT_MAX
+| SvDT_MIN
+| SvDT_PRINT
+
+val state_var_eq : stateVar -> stateVar -> bool
+
+val svIndex : stateVar -> positive
+
+val svStrList : (stateVar * char list) list
+
+module SvIndex :
+ sig
+  type t = stateVar
+
+  val index : stateVar -> positive
+
+  val eq : stateVar -> stateVar -> bool
+ end
+
+module SvTree :
+ sig
+  type elt = SvIndex.t
+
+  val elt_eq : SvIndex.t -> SvIndex.t -> bool
+
+  type 'x t = 'x PTree.t
+
+  val empty : 'a1 t
+
+  val get : elt -> 'a1 t -> 'a1 option
+
+  val set : elt -> 'a1 -> 'a1 t -> 'a1 t
+
+  val remove : elt -> 'a1 t -> 'a1 t
+
+  val beq : ('a1 -> 'a1 -> bool) -> 'a1 t -> 'a1 t -> bool
+
+  val combine : ('a1 option -> 'a2 option -> 'a3 option) -> 'a1 t -> 'a2 t -> 'a3 t
+ end
+
+type stringSvTreeTy = char list SvTree.t
+
+val emptyStringPTree : char list SvTree.t
+
+val updateStringSvTree : (stateVar * char list) list -> stringSvTreeTy -> stringSvTreeTy
+
+val svToStringTree : stringSvTreeTy
+
+val svToStrOpt : stateVar -> char list option
+
+val svToStr : stateVar -> char list
+
+type floatSvTreeTy = float SvTree.t
+
+val emptyFloatPTree : float SvTree.t
+
+val updateFloatSvTree : (stateVar * float) list -> floatSvTreeTy -> floatSvTreeTy
+
+val stringKeyValToFloatKeyVal : (stateVar * char list) list -> (stateVar * float) list
+
+val driver_defaults_str : (stateVar * char list) list
+
+val driver_defaults : unit -> (stateVar * float) list
+
+val model_default_values_str : (stateVar * char list) list
+
+val model_default_values : unit -> (stateVar * float) list
+
+val state0 : unit -> floatSvTreeTy
+
+val svGetFloat : stateVar -> floatSvTreeTy -> float
+
+val modelOutputs : stateVar list
+
+type flagsTy = { stop_simulation : bool; end_of_run : bool; evaluate_xd : bool }
+
+val stop_simulation : flagsTy -> bool
+
+val end_of_run : flagsTy -> bool
+
+val evaluate_xd : flagsTy -> bool
+
+type eventFuncId =
+| EfiStop
+| EfiAppendSolution
+| EfiTerminateSim
+| EfiFlip_Xd_At_Bounce
+
+type eventTy = { key : char list; time : float; func : eventFuncId }
+
+val key : eventTy -> char list
+
+val time : eventTy -> float
+
+val func : eventTy -> eventFuncId
+
+type logEntryTy = { le_caption : char list; le_vars : (char list * char list) list;
+                    le_events : (char list * char list) list }
+
+type simTy = { vars : floatSvTreeTy; solkeys : stateVar list; solution : char list list list;
+               sim_events : eventTy list; log : logEntryTy list; flags : flagsTy }
+
+val vars : simTy -> floatSvTreeTy
+
+val solkeys : simTy -> stateVar list
+
+val solution : simTy -> char list list list
+
+val sim_events : simTy -> eventTy list
+
+val log : simTy -> logEntryTy list
+
+val flags : simTy -> flagsTy
+
+val log_sim : char list -> simTy -> simTy
+
+val default_flags : flagsTy
+
+val t_ge_tstop_event_func : eventTy -> simTy -> simTy * float option
+
+val make_solution_row_helper : floatSvTreeTy -> stateVar list -> char list list
+
+val make_solution_row : simTy -> simTy
+
+val append_solution_event_func : eventTy -> simTy -> simTy * float option
+
+val terminate_sim_event_func : eventTy -> simTy -> simTy * float option
+
+val driver_default_events : eventTy list
+
+val default_sim : simTy
+
+val default_sim_log : simTy
+
+val f99 : float
+
+val bounceEvent : eventTy
+
+val init_sim : simTy -> simTy
+
+val set_vars : simTy -> floatSvTreeTy -> simTy
+
+val flip_xd_at_bounce_event_func : eventTy -> simTy -> simTy * float option
+
+val handle_event : eventTy -> simTy -> simTy * float option
+
+val set_var : stateVar -> float -> simTy -> simTy
+
+val fhalf : float
+
+val ftwo : float
+
+val epsilon : float
+
+val efi_eqb : eventFuncId -> eventFuncId -> bool
+
+val schedule_event : eventTy list -> eventFuncId -> float -> eventTy list
+
+val sqrt : float -> float
+
+val fone : float
+
+val differential_equations : simTy -> simTy
+
+val zofFloat : float -> z
+
+val round : float -> float
+
+val tenTo6 : float
+
+val process_one_event : eventTy -> simTy -> eventTy * simTy
+
+val process_events_helper : eventTy list -> simTy -> eventTy list * simTy
+
+val min_event_time : eventTy list -> float -> float
+
+val process_events : simTy -> simTy
+
+val advance_states : (stateVar * stateVar) list -> float -> simTy -> simTy
+
+val advance_model : simTy -> simTy
+
+val oneStep : simTy -> simTy
+
+val run_sim_loop : z -> simTy -> simTy
+
+val run_sim : simTy -> simTy
+
+val sim_in : unit -> simTy
+
+val main : unit -> simTy
