formal/coqimp/print_digsim.ml
@@ -1,0 +1,35 @@
+open Top
+open Debug_printers
+open DebugIO
+open Maps
+
+let char_list_to_string cl = String.init (List.length cl) (fun i -> (List.nth cl i));;
+
+let print_svtree tree =
+  Format.printf "@[SvFloatTree@,";
+  let kvpairs = PTree.elements tree in
+  List.map (fun (pos, fval) ->
+      let sv = posToStateVar' pos in
+      let svstring = char_list_to_string (svToStr sv) in
+      let fstr = char_list_to_string (DebugIO.print_float fval) in
+      Format.printf "@[(%s ->@ %s)@]" svstring fstr)
+    kvpairs;
+  Format.printf "@]";;
+
+
+(* 
+
+For ocaml top level:
+
+#install_printer my_print_z;;
+#install_printer my_print_float;; 
+#install_printer my_char_list;;
+
+For ocamldebug:
+
+install_printer My_printers.my_print_z
+install_printer My_printers.my_print_float
+install_printer My_printers.my_print_char_list
+
+ *)
+
