formal/diguty/my_printers.ml
@@ -1,0 +1,28 @@
+open Float_text_io
+open FloatIO
+open Debug_printers
+open DebugIO
+
+let char_list_to_string cl = String.init (List.length cl) (fun i -> (List.nth cl i));;
+let char_list_to_string_quoted cl = "\"" ^ (char_list_to_string cl) ^ "\"";;
+let my_print_z z = Format.print_string (char_list_to_string (print_Z z));;
+
+let my_print_float x = Format.print_string (char_list_to_string (print_float x));;
+
+let my_print_char_list (cl: char list) = Format.print_string (char_list_to_string_quoted cl);;
+(* 
+
+For ocaml top level:
+
+#install_printer my_print_z;;
+#install_printer my_print_float;; 
+#install_printer my_char_list;;
+
+For ocamldebug:
+
+install_printer My_printers.my_print_z
+install_printer My_printers.my_print_float
+install_printer My_printers.my_print_char_list
+
+ *)
+
