formal/coqimp/digsim5x.v
@@ -1,0 +1,868 @@
+(** DigSim
+
+   DigSim provides a Coq architecture required to simulate continuous systems
+   described by sets of simultaneous first-order differential equations.
+
+     xdd := -(spring_coefficient*x + damping_coefficient*xd)/mass - gravity;
+
+
+ ** _CoqProject config file contents
+
+   -R ~/opt/lib/compcert/coq compcert -R . Top
+
+ *)
+
+From RecordUpdate Require Import RecordUpdate.
+Module RecordSetNotations'.
+  Delimit Scope record_set with rs.
+  Open Scope rs.
+  (*
+    Note that the "set" function, after the proj argument, takes a function from 
+    the old value to the new value. "(constructor v)" will make such a function
+    that will ignore the old value and return v.
+  *)
+  Notation "x [[ proj  :=  v ]]" := (set proj (constructor v) x)
+                                    (at level 12, left associativity) : record_set.
+  Notation "x [[ proj  ::=  f ]]" := (set proj f x)
+                                     (at level 12, f at next level, left associativity) : record_set.
+End RecordSetNotations'.
+Import RecordSetNotations'.
+
+Require Import DigUty.float_text_io.
+Import FloatIO.
+Require Import DigUty.debug_printers.
+Import DebugIO.
+
+Require Import DigUty.Monad.
+
+From compcert Require Import Floats.
+Import Float.
+From compcert Require Import Fappli_IEEE.
+From compcert Require Import Integers.
+Require Import Coq.Lists.List.
+
+Import ListNotations.
+
+Require Import BinNums.
+Require Import Coq.QArith.QArith_base.
+Require Import Strings.String.
+Require Import Strings.Ascii.
+Require Import Coq.ZArith.Znat.
+Require Import Recdef.
+From compcert Require Import Maps.
+
+(* Inductive type used to name state variables. *)
+Inductive stateVar : Set := 
+| SvT
+| SvX
+| SvXD
+| SvXDD
+| SvCOEFF_OF_REST
+| SvGRAVITY
+| SvT_STOP
+| SvDT
+| SvDT_MAX
+| SvDT_MIN
+| SvDT_PRINT.
+
+Lemma state_var_eq: forall (r1 r2: stateVar), {r1 = r2} + {r1 <> r2}.
+Proof. decide equality. Defined.
+Global Opaque state_var_eq.
+
+From compcert Require Import Decidableplus.
+
+Instance Decidable_eq_sv : forall (x y: stateVar), Decidable (eq x y) := Decidable_eq state_var_eq.
+
+(* For diagnostic purposes we want to map from the positive id for a
+   stateVar to the stateVar. 
+ *)
+Definition posToStateVarTreeType := PTree.t stateVar.
+Definition emptyPosToStateVarTree := PTree.empty stateVar.
+
+Definition svIndex (sv: stateVar) : positive :=
+  match sv with
+  | SvT => 1
+  | SvX => 2
+  | SvXD => 3
+  | SvXDD => 4
+  | SvCOEFF_OF_REST => 5
+  | SvGRAVITY => 6
+  | SvT_STOP => 7
+  | SvDT => 8
+  | SvDT_MAX => 9
+  | SvDT_MIN => 10
+  | SvDT_PRINT => 11
+  end.
+
+Definition svStrList :=
+  [
+    (SvT, "T");
+    (SvX, "X");
+    (SvXD, "XD");
+    (SvXDD, "XDD");
+    (SvCOEFF_OF_REST, "COEFF_OF_REST");
+    (SvGRAVITY, "GRAVITY");
+    (SvT_STOP, "T_STOP");
+    (SvDT, "DT");
+    (SvDT_MAX, "DT_MAX");
+    (SvDT_MIN, "DT_MIN");
+    (SvDT_PRINT, "DT_PRINT")
+  ]%positive.
+
+Fixpoint updatePosToStateVarTree (svIdStrList: list (stateVar * string))
+         (tree: posToStateVarTreeType) : posToStateVarTreeType :=
+  match svIdStrList with
+  | nil => tree
+  | cons (sv, str) xtail =>
+    let tree1 := PTree.set (svIndex sv) sv tree in
+    updatePosToStateVarTree xtail tree1
+  end.
+
+Definition posToStateVarTree :=
+  (* Eval compute in *) updatePosToStateVarTree svStrList emptyPosToStateVarTree.
+
+Definition posToStateVar (p: positive) := PTree.get p posToStateVarTree.
+
+(*
+Compute PTree.elements posToStateVarTree.
+Compute posToStateVar 3.
+*)
+
+Module SvIndex <: Maps.INDEXED_TYPE.
+  Definition t := stateVar.
+  Definition index := svIndex.
+  Definition eq := state_var_eq.
+  Lemma index_inj:
+    forall r1 r2, index r1 = index r2 -> r1 = r2.
+  Proof.
+    intros.
+    destruct r1 eqn: r1eq; destruct r2 eqn: r2eq; simpl in *;try reflexivity;
+      unfold index in H; simpl in H; inversion H.
+  Qed.
+End SvIndex.
+
+Module SvTree := Maps.ITree(SvIndex).
+
+Definition stringSvTreeTy := SvTree.t string.
+Definition emptyStringPTree := SvTree.empty string.
+
+Fixpoint updateStringSvTree (valList: list (stateVar * string)) (intree: stringSvTreeTy) :=
+  match valList with
+  | nil => intree
+  | cons (sv, val) vltail =>
+    let tree1 := SvTree.set sv val intree in
+    updateStringSvTree vltail tree1
+  end.
+
+Definition svToStringTree :=
+  (* Eval compute in *) updateStringSvTree svStrList emptyStringPTree.
+
+Definition svToStrOpt (sv: stateVar) : option string :=
+  SvTree.get sv svToStringTree.
+
+Lemma svToStrComplete:
+  forall sv : stateVar, exists s : string,
+      svToStrOpt sv = Some s.
+Proof.
+  intros.
+  destruct sv; unfold svToStrOpt;compute; eexists; f_equal.
+Qed.
+
+(* Since we have proven that svToStrOpt will always give a 
+   result, define a function that extracts that value,
+   and in the impossible case returns the empty string.
+*)
+Definition svToStr (sv: stateVar) : string :=
+  match svToStrOpt sv with
+  | Some x => x
+  | None => ""
+  end.
+
+(*
+Compute svToStr SvDT.
+Compute svToStr SvDT_PRINT.
+*)
+
+Definition floatSvTreeTy := SvTree.t float.
+Definition emptyFloatPTree := SvTree.empty float.
+
+Fixpoint updateFloatSvTree (valList: list (stateVar * float)) (intree: floatSvTreeTy) :=
+  match valList with
+  | nil => intree
+  | cons (sv, fval) vltail =>
+    let tree1 := SvTree.set sv fval intree in
+    updateFloatSvTree vltail tree1
+  end.
+
+(* Take state variable string pairs and convert to 
+   state variable float pairs, by converting each
+   string into a float. If the string cannot be converted,
+   then skip it.
+*)
+Fixpoint stringKeyValToFloatKeyVal (kvl: list (stateVar * string)) : list (stateVar * float) :=
+  match kvl with
+  | nil => nil
+  | cons (sv, str) tl =>
+    let tailkvs := stringKeyValToFloatKeyVal tl in
+    match strToFloat str with
+    | Some fval => (sv, fval) :: tailkvs
+    | None => tailkvs
+    end
+  end.
+
+Fixpoint printFloatKeyVals (kvl: list (stateVar * float)) :=
+  match kvl with
+  | nil => nil
+  | cons (sv, fval) tl =>
+    (sv, print_float fval) :: printFloatKeyVals tl
+  end.
+
+Definition driver_defaults_str :=
+  [
+            (SvT,        "0.0");
+            (SvT_STOP,   "0.0");
+            (SvDT,       "0.005");
+            (SvDT_MAX,   "0.005");
+            (SvDT_MIN,   "0.005");
+            (SvDT_PRINT, "0.01")
+  ].
+
+Definition driver_defaults (_ : unit) :=
+  (* Eval compute in *) stringKeyValToFloatKeyVal driver_defaults_str.
+
+(* Compute printFloatKeyVals driver_defaults. *)
+
+Definition model_default_values_str :=
+  [
+    (SvT,             "0.0");
+    (SvX,             "10.0");
+    (SvXD,            "0.0");
+    (SvXDD,           "0.0");
+    (SvCOEFF_OF_REST, "0.80");
+    (SvGRAVITY,       "9.88");
+    (SvT_STOP,        "10.0");
+    (SvDT,            "0.01");
+    (SvDT_MAX,        "0.005");
+    (SvDT_MIN,        "0.001");
+    (SvDT_PRINT,      "0.01")
+  ].
+
+Definition model_default_values (_ : unit) :=
+  (* Eval compute in *) stringKeyValToFloatKeyVal model_default_values_str.
+
+(* Compute printFloatKeyVals model_default_values. *)
+
+Definition state0 (_ : unit) := (* Eval compute in *)
+      let driverState := updateFloatSvTree (driver_defaults tt) emptyFloatPTree in
+      updateFloatSvTree (model_default_values tt) driverState.
+
+Definition svToFloat0 (sv: stateVar) := SvTree.get sv (state0 tt).
+
+Definition svToFloatStr0 (sv: stateVar) :=
+  match svToFloat0 sv with
+  | Some x => print_float x
+  | None => "None"
+  end.
+
+(* Compute svToFloatStr0 SvGRAVITY. *)
+
+(* Takes a long time.
+Lemma state0Complete:
+  forall sv: stateVar, exists f: float,
+      SvTree.get sv (state0 ()) = Some f.
+Proof.
+  intros.
+  destruct sv;compute; eexists; f_equal.
+Qed.
+ *)
+
+(* Since we have proven that state is complete, we can define a
+   function that always returns a float, using a default
+   in the impossible case.
+ *)
+Definition svGetFloat (sv: stateVar) (tree : floatSvTreeTy) :=
+  match SvTree.get sv tree with
+  | Some x => x
+  | None => 0%D
+  end.
+
+(* Compute PTree.elements (state0 ()). *)
+
+
+(* Give stateVar given its positive id, or if not a valid id,
+   an arbitrary stateVar
+*)
+Definition posToStateVar' (pos: positive) :=
+  match posToStateVar pos with
+  | Some x => x
+  | None => SvT
+  end.
+
+Fixpoint printFloatStateElements (elist: list (positive * float)) : list (string * string) :=
+  match elist with
+  | nil => nil
+  | cons (pos, fval) tl =>
+    (svToStr (posToStateVar' pos), print_float fval) :: printFloatStateElements tl
+  end.
+
+Definition printFloatState (state: floatSvTreeTy) :=
+  printFloatStateElements (PTree.elements state).
+
+(* Compute printFloatState (state0 ()). *)
+
+(*
+Compute float_to_string 8 4 (svGetFloat SvGRAVITY (state0 ())).
+Compute SvTree.get SvXD (SvTree.set SvXD 0%D emptyFloatPTree).
+*)
+
+Definition modelOutputs : list stateVar := [SvT; SvX; SvXD].
+Print modelOutputs.
+
+Record flagsTy :=
+  mkFlags
+    {
+      stop_simulation : bool; (* Stop the simulation, t > tStop, *)
+      end_of_run : bool;      (* Terminate early, user event logic. *)
+      evaluate_xd : bool     (* Flag to determine of xd needs to reevaluated. *)
+    }.
+
+Instance etaFlags  : Settable _ := 
+  mkSettable (constructor mkFlags
+                          <*> stop_simulation
+                          <*> end_of_run
+                          <*> evaluate_xd
+             )%set.
+
+Inductive eventFuncId :=
+| efiStop
+| efiAppendSolution
+| efiTerminateSim
+| efiFlip_Xd_At_Bounce
+.
+
+Record eventTy :=
+  mkEvent
+    {
+      key : string;
+      time : float;
+      func : eventFuncId
+    }.
+
+Instance etaEvent : Settable eventTy := 
+  mkSettable (constructor mkEvent
+                          <*> key
+                          <*> time
+                          <*> func
+             )%set.
+
+Record logEntryTy :=
+  mkLogEntry
+    {
+      le_caption: string;
+      le_vars: list (string * string);
+      le_events: list (string * string);
+    }.
+
+Instance etaLogEntry : Settable _ :=
+  mkSettable (constructor mkLogEntry
+                          <*> le_caption
+                          <*> le_vars
+                          <*> le_events
+             )%set.
+
+Record simTy :=
+  mkSim
+    {
+      vars : floatSvTreeTy;              (* Simulation variables and constants. *)
+      solkeys : list stateVar;         (* Keys of fields in Solution. *)
+      solution : list (list string);   (* Simulation detail results. *)
+      sim_events : list eventTy;   (* User events. *)
+      log : list logEntryTy;               (* Text logging for debugging or information. *)
+      flags : flagsTy                    (* control flags *)
+    }.
+
+Instance etaSim  : Settable _ := 
+  mkSettable (constructor mkSim
+                          <*> vars
+                          <*> solkeys
+                          <*> solution
+                          <*> sim_events
+                          <*> log
+                          <*> flags
+             )%set.
+
+Definition printFloatSvTreeTy (vars: floatSvTreeTy) :=
+  printFloatStateElements (PTree.elements vars).
+
+Fixpoint logEvents (evs: list eventTy) : list (string * string) :=
+  match evs with
+  | nil => nil
+  | cons ev evtl =>
+    let caption := ev.(key) in
+    let time_str := print_float ev.(time) in
+    (caption, time_str) :: logEvents evtl
+  end.
+
+(* Use this version if you want a log 
+Definition log_sim (caption: string) (sim: simTy) : simTy :=
+  let le := {|
+        le_caption := caption;
+        le_vars := printFloatSvTreeTy sim.(vars);
+        le_events := logEvents sim.(sim_events)
+      |} in
+  let result_sim := sim[[log ::= (fun oldlog => le :: oldlog)]] in
+  result_sim.
+
+ *)
+
+(* This is the dummy version *)
+Definition log_sim (caption: string) (sim: simTy) : simTy := sim.
+
+Definition default_flags :=
+  {|
+    stop_simulation := false;
+    end_of_run := false;
+    evaluate_xd := false;
+  |}.
+
+(* Return value is a pair of the updated sim, and an optional float which,
+   if present, is the new time at which the event should be scheduled.
+   The caller must do this.
+ *)
+Open Scope D_scope.
+
+Definition t_ge_tstop_event_func (this: eventTy) (sim: simTy) : (simTy * option float) :=
+  let sim1 := log_sim "t_ge_tstop_event_func: sim1" sim in
+  let vars := sim1.(vars) in
+  let t := svGetFloat SvT vars in
+  let t_stop := svGetFloat SvT_STOP vars in
+  let stop_sim := t >=? t_stop in
+  let new_flags := sim1.(flags)[[stop_simulation := stop_sim]] in
+  let result_sim := sim1[[flags := new_flags]] in
+  let result_log := log_sim "t_ge_tstop_event_func: result_sim" result_sim in
+  (result_log, None).
+
+Fixpoint make_solution_row_helper (vars: floatSvTreeTy) (keys: list stateVar) : list string :=
+  match keys with
+  | nil => nil
+  | cons key others =>
+    let fval := svGetFloat key vars in
+    let sval := print_float fval in
+    sval :: make_solution_row_helper vars others
+  end.
+
+Definition make_solution_row (sim: simTy) :=
+  let row := make_solution_row_helper sim.(vars) sim.(solkeys) in
+  let result_sim := sim[[solution ::= (fun old => row :: old)]] in
+  let result_log := log_sim "make_solution_row: result" result_sim in
+  result_log.
+
+Definition append_solution_event_func (this: eventTy) (sim: simTy) : (simTy * option float) :=
+  let sim1 := make_solution_row sim in
+  let sim1log := log_sim "append_solution_event_func:sim1" sim1 in
+  let vars := sim1log.(vars) in
+  let dt_print := svGetFloat SvDT_PRINT vars in
+  let t := svGetFloat SvT vars in
+  let new_t := t + dt_print in
+  (sim1log, Some new_t).
+
+Definition terminate_sim_event_func (this: eventTy) (sim: simTy) : (simTy * option float) :=
+  let simlog := log_sim "terminate_sim_event_func: sim" sim in
+  (simlog, None).
+
+Definition driver_default_events :=
+  [
+    {| key := "t_ge_tstop_event"; time := 0%D; func := efiStop|};
+    {| key := "append_log_event"; time := 0%D; func := efiAppendSolution|};
+    {| key := "terminate_sim_event"; time := 0%D; func := efiTerminateSim|}
+  ].
+
+Definition default_sim :=
+  {|
+    vars := (state0 tt);
+    solkeys := modelOutputs;
+    solution := nil;
+    sim_events := driver_default_events;
+    log := nil;
+    flags := default_flags;
+  |}.
+
+Definition default_sim_log:= log_sim "default_sim" default_sim.
+
+Definition f99 := (* Eval compute in *) strToFloat' "99.0".
+
+Definition bounceEvent :=
+  {| key := "flip_xd_at_bounce_event";
+     time := f99;
+     func := efiFlip_Xd_At_Bounce;
+  |}.
+
+Definition init_sim (sim: simTy) :=
+  let sim' := log_sim "init_sim:sim" sim in
+  let result_sim := sim[[sim_events ::= (fun evs => bounceEvent :: evs)]] in
+  let result_sim' := log_sim "init_sim: result" result_sim in
+  result_sim'.
+
+Definition set_vars (sim: simTy) (new_vars : floatSvTreeTy) :=
+  let sim' := log_sim "set_vars:sim" sim in
+  let new_vars' := printFloatSvTreeTy new_vars in
+  let result_sim := sim[[vars := new_vars]] in
+  let result_sim' := log_sim "set_vars: result" result_sim in
+  result_sim'.
+
+
+Definition flip_xd_at_bounce_event_func (this: eventTy) (sim: simTy) : (simTy * option float) :=
+  let sim' := log_sim "flip_xd_at_bounce_event_func: sim" sim in
+  let vars := sim'.(vars) in
+  let coeff_of_rest := svGetFloat SvCOEFF_OF_REST vars in
+  let xd := svGetFloat SvXD vars in
+  let new_xd := - (coeff_of_rest * xd) in
+  let vars' := SvTree.set SvXD new_xd vars in
+  let new_flags := sim'.(flags)[[evaluate_xd := true]] in
+  let sim2 := set_vars sim' vars' in
+  let result_sim := sim2[[flags := new_flags]] in
+  let result_log := log_sim "flip_xd_at_bounce_event_func" result_sim in
+  (result_log, Some f99).
+
+Definition handle_event (this: eventTy) (sim: simTy) : (simTy * option float) :=
+  let sim_log := log_sim "handle_event:sim" sim in
+  let result := 
+      match this.(func) with
+      | efiStop => t_ge_tstop_event_func this sim_log
+      | efiAppendSolution => append_solution_event_func this sim_log
+      | efiTerminateSim => terminate_sim_event_func this sim_log
+      | efiFlip_Xd_At_Bounce => flip_xd_at_bounce_event_func this sim_log
+      end in
+  let (result_sim, maybefloat) := result in
+  let result_log := log_sim "handle_event:result" result_sim in
+  (result_log, maybefloat).
+
+Definition set_var (key: stateVar) (val: float) (sim: simTy) :=
+  let sim_log := log_sim "set_var:sim" sim in
+  let result_sim := sim_log[[vars := SvTree.set key val sim.(vars)]] in
+  let result_log := log_sim "set_var:result" result_sim in
+  result_log.
+
+Definition fhalf := (* Eval compute in *) strToFloat' "0.5".
+Definition ftwo := (* Eval compute in *) strToFloat' "2.0".
+
+(* pi matching Haskell Prelude Double *)
+Definition pi := (* Eval compute in *) strToFloat' "3.141592653589793238".
+
+(* small floating point constant *)
+Definition small := (* Eval compute in *) strToFloat' "0.000001".
+
+(* comparison floating point constant *)
+Definition epsilon := (* Eval compute in *) strToFloat' "0.0000000001".
+(* Compute float_to_string 0 19 pi. *)
+
+Definition efi_eqb (fi1 fi2 : eventFuncId) : bool :=
+  match fi1, fi2 with
+  | efiStop, efiStop => true
+  | efiAppendSolution, efiAppendSolution => true
+  | efiTerminateSim, efiTerminateSim => true
+  | efiFlip_Xd_At_Bounce, efiFlip_Xd_At_Bounce => true
+  | _, _ => false
+  end.
+
+(* Update a list of events by changing the scheduled time for the 
+   one with the specified function id.
+*)
+Fixpoint schedule_event (evs: list eventTy) (efi: eventFuncId) (new_time: float) :=
+  match evs with
+  | nil => nil
+  | cons ev evtl =>
+    let ev' :=
+        if efi_eqb ev.(func) efi then
+          ev[[time := new_time]]
+        else
+          ev
+    in
+    ev' :: schedule_event evtl efi new_time
+  end.
+
+Definition sqrt (arg: float) : float :=
+  Fappli_IEEE_bits.b64_sqrt mode_NE arg.
+(*
+Definition F9 := (* Eval compute in *) strToFloat' "9.0".
+Definition sqrt9 := (* Eval compute in *) sqrt F9.
+Compute print_float sqrt9.
+ *)
+
+Definition fone := (* Eval compute in *) strToFloat' "1.0".
+
+Definition differential_equations (sim: simTy) : simTy :=
+  let sim_log := log_sim "differential_equations" sim in
+  let vars := sim_log.(vars) in
+  let t := svGetFloat SvT vars in
+  let x := svGetFloat SvX vars in
+  let xd := svGetFloat SvXD vars in
+  let dt_min := svGetFloat SvDT_MIN vars in
+  let dt_max := svGetFloat SvDT_MAX vars in
+  let gravity := svGetFloat SvGRAVITY vars in
+  let t_stop := svGetFloat SvT_STOP vars in
+
+  let xdd := -gravity in
+  let sim1 := set_var SvXDD xdd sim_log in
+  let sim1log := log_sim "differential_equations:sim1" sim1 in
+  let est_max := x + xd * dt_max + fhalf * xdd * dt_max * dt_max in
+  let dt_impact := t_stop + fone in
+  let dt_impact2 :=
+      if (est_max <=? 0%D) then
+        let est_min := x + xd * dt_min + fhalf * xdd * dt_min * dt_min in
+        if (est_min <=? 0%D) then
+            0%D
+        else
+            let dt_impact3 := (-xd - sqrt(xd * xd - ftwo * x * xdd)) / (ftwo * x) in
+            if (dt_min - dt_impact3 >? epsilon) then
+              (-xd + sqrt(xd * xd - ftwo * x * xdd)) / (ftwo * x)
+            else
+              dt_impact3
+      else
+        dt_impact in
+  let impact_time := t + dt_impact2 in
+  let events' := schedule_event sim1log.(sim_events) efiFlip_Xd_At_Bounce impact_time in
+  let result_sim := sim1log[[sim_events := events']] in
+  let result_log := log_sim "differential_equations" result_sim in
+  result_log.
+
+Definition ZofFloat (f: float) :=
+  match Fappli_IEEE_extra.ZofB 53 1024 f with
+  | Some z => z
+  | None => 0%Z
+  end.
+
+Definition round (f: float) : float :=
+  let z := ZofFloat (f + fhalf) in
+  Z_to_float z.
+
+Definition tenTo6 := (* Eval compute in *) strToFloat' "1.e6".
+
+Definition process_one_event (ev: eventTy) (sim: simTy) :=
+  let sim_log := log_sim "process_one_event:sim" sim in
+  let vars := sim_log.(vars) in
+  let t := svGetFloat SvT vars in
+  let dt_min := svGetFloat SvDT_MIN vars in
+  let dt_max := svGetFloat SvDT_MAX vars in
+  let et := ev.(time) in
+  let etdelta := round ((et - t) * tenTo6) in
+  let minrnd := round (dt_min * tenTo6) in
+  let (ev', result_sim) :=
+      if (etdelta <? minrnd) then
+        let (sim2, new_time_opt) := handle_event ev sim_log in
+        let sim2log := log_sim "process_one_event:sim2" sim2 in
+        match new_time_opt with
+        | Some new_time => (ev[[time := new_time]], sim2log)
+        | None => (ev, sim2log)
+        end
+      else
+        (ev, sim_log)
+  in
+  let result_log := log_sim "process_one_event" result_sim in
+  (ev', result_log).
+
+Fixpoint process_events_helper (evs: list eventTy) (sim: simTy) :=
+  match evs with
+  | nil => (nil, sim)
+  | cons ev evtl =>
+    let (ev', sim') := process_one_event ev sim in
+    let (evs', sim'') := process_events_helper evtl sim' in
+    (ev' :: evs', sim'')
+  end.
+
+Fixpoint min_event_time (evs: list eventTy) (min_so_far: float) : float :=
+  match evs with
+  | nil => min_so_far
+  | cons ev evtl =>
+    let et := ev.(time) in
+    let new_min :=
+        if (et >? 0%D) && (et <? min_so_far) then
+          et
+        else
+          min_so_far
+    in
+    min_event_time evtl new_min
+  end.
+
+  
+Definition process_events (sim: simTy) : simTy :=
+  let sim_log := log_sim "process_events:sim" sim in
+  let vars0 := sim_log.(vars) in
+  let events := sim_log.(sim_events) in
+  let result_sim := 
+      match events with
+      | nil => set_var SvDT (svGetFloat SvDT_MAX vars0) sim_log
+      | cons x x0 =>
+        let t := svGetFloat SvT vars0 in
+        let dt_max := svGetFloat SvDT_MAX vars0 in
+        let (evs', sim1) := process_events_helper events sim_log in
+        let sim1log := log_sim "process_events:sim1" sim1 in
+        let vars' := sim1log.(vars) in
+        let min_time0 := svGetFloat SvT_STOP vars' in
+        let min_time := min_event_time evs' min_time0 in
+        let time_to_next_event := min_time - t in
+        let new_dt :=
+            if (time_to_next_event >? 0%D) && ((dt_max - time_to_next_event) >? epsilon) then
+              time_to_next_event
+            else 
+              dt_max
+        in
+        let sim3 := set_var SvDT new_dt sim1log in
+        let sim4 := sim3[[sim_events := evs']] in
+        let sim4log := log_sim "process_events:sim4" sim4 in
+        sim4log
+      end in
+  let result_log := log_sim "process_events:result" result_sim in
+  result_log.
+
+Fixpoint advance_states (pairs: list (stateVar * stateVar)) (dt: float) (sim: simTy) : simTy :=
+  let sim_log := log_sim "advance_states:sim" sim in
+  let result_sim := 
+      match pairs with
+      | nil => sim
+      | cons (sv, svd) pairstl =>
+        let vars0 := sim.(vars) in
+        let el := svGetFloat sv vars0 in
+        let eld := svGetFloat svd vars0 in
+        let el' := el + eld * dt in
+        let sim1 := set_var sv el' sim in
+        let sim1log := log_sim "advance_states:sim1" sim1 in
+        let sim2 := advance_states pairstl dt sim1log in
+        sim2
+      end in
+  let result_log := log_sim "advance_states:result" result_sim in
+  result_log.
+
+Definition advance_model (sim: simTy) : simTy :=
+  let sim_log := log_sim "advance_model:sim" sim in
+  let vars0 := sim_log.(vars) in
+  let dt := svGetFloat SvDT vars0 in
+  let pairs := [(SvX, SvXD); (SvXD, SvXDD) ] in
+  let sim2 := advance_states pairs dt sim_log in
+  let sim2log := log_sim "advance_model:sim2" sim2 in
+  let vars' := sim2log.(vars) in
+  let t := svGetFloat SvT vars' in
+  let new_t := t + dt in
+  let rounded_new_t := round (new_t * tenTo6)/tenTo6 in
+  (* let rounded_new_t := new_t in *)
+  let result_sim := set_var SvT rounded_new_t sim2log in
+  let result_log := log_sim "advance_model:result" result_sim in
+  result_log.
+
+Definition oneStep (sim: simTy) : simTy :=
+  let sim_log := log_sim "oneStep:sim" sim in
+  let sim1 := differential_equations sim_log in
+  let sim1log := log_sim "oneStep:sim1" sim1 in
+  let sim2 := process_events sim1log in
+  let sim2log := log_sim "oneStep:sim2" sim2 in
+  let sim3 :=
+      if sim2log.(flags).(evaluate_xd) then
+        let sim4 := differential_equations sim2log in
+        let sim4log := log_sim "oneStep:sim4" sim4 in
+        let flags4 := sim4log.(flags) in
+        let flags4' := flags4[[evaluate_xd := false]] in
+        let sim6 := sim4log[[flags := flags4']] in
+        let sim6log := log_sim "oneStep:sim6" sim6 in
+        sim6log
+      else
+        sim2log in
+  let sim3log := log_sim "oneStep:sim3" sim3 in
+  let sim5 := advance_model sim3log in
+  let sim5log := log_sim "oneStep:sim5" sim5 in
+  sim5log.
+
+Require Import Zwf.
+From compcert Require Import Coqlib.
+
+Function run_sim_loop (steps: Z) (sim: simTy) { wf (Zwf 0%Z) steps } :=
+  let result_sim := 
+      if zle 0%Z steps
+      then
+        let f := sim.(flags) in
+        if f.(end_of_run) || f.(stop_simulation)
+        then sim
+        else
+          let sim2 := (oneStep sim) in
+          (* let sim2log := log_sim "run_sim_loop:sim2" sim2 in *)
+          let steps2 := (steps - 1) in 
+          run_sim_loop steps2 sim2
+      else sim
+  in
+  result_sim.
+Proof.
+  intros; red; omega.
+  apply Zwf_well_founded.
+Qed.
+
+(*
+Definition binary64 := binary_float 53 1024.
+*)
+
+Definition run_sim (sim: simTy) :=
+  let sim_log := log_sim "run_sim:sim" sim in
+  let vars := sim_log.(vars) in
+  let dtmin := svGetFloat SvDT_MIN vars in
+  let tstop := svGetFloat SvT_STOP vars in
+  let max_steps_float := (tstop / dtmin)%D in
+  let steps := ZofFloat max_steps_float in
+  let result_sim := run_sim_loop steps sim_log in
+  let result_log := log_sim "run_sim:result" result_sim in
+  result_log.
+
+Definition sim_in (_ : unit) :=
+  let sim1 := default_sim_log in
+  let sim1log := log_sim "sim_in:sim1" sim1 in
+  let sim2 := init_sim sim1log in
+  let sim2log := log_sim "sim_in:sim2" sim2 in
+  let sim3 := set_var SvCOEFF_OF_REST (strToFloat' "0.80") sim2log in
+  let sim3log := log_sim "sim_in:sim3" sim3 in
+  let sim4 := set_var SvGRAVITY (strToFloat' "9.88") sim3log in
+  let sim4log := log_sim "sim_in:sim4" sim4 in
+  sim4log.
+
+Definition main (_ : unit) :=
+  let sim1 := (sim_in tt) in
+  let sim1log := log_sim "sim_main:sim1" sim1 in
+  let sim2 := run_sim  sim1 in
+  let sim2log := log_sim "sim_main:result" sim2 in
+  let sim3 := sim2log[[solution ::= (fun sol => rev sol)]] in
+  let sim4 := sim3[[log ::= (fun lg => rev lg)]] in
+  sim4.
+
+Extraction Language OCaml.
+(* Unset Extraction Optimize. *)
+(* Unset Extraction AutoInline. *)
+
+(* Standard lib *)
+Require Import ExtrOcamlBasic.
+Require Import ExtrOcamlString.
+
+(* Coqlib *)
+Extract Inlined Constant Coqlib.proj_sumbool => "(fun x -> x)".
+
+(* Datatypes *)
+Extract Inlined Constant Datatypes.fst => "fst".
+Extract Inlined Constant Datatypes.snd => "snd".
+
+(* Decidable *)
+
+Extraction Inline DecidableClass.Decidable_witness DecidableClass.decide
+   Decidableplus.Decidable_and Decidableplus.Decidable_or
+   Decidableplus.Decidable_not Decidableplus.Decidable_implies.
+
+(* Avoid name clashes *)
+Extraction Blacklist List String Int.
+
+(* Cutting the dependency to R. *)
+Extract Inlined Constant Fcore_defs.F2R => "fun _ -> assert false".
+Extract Inlined Constant Fappli_IEEE.FF2R => "fun _ -> assert false".
+Extract Inlined Constant Fappli_IEEE.B2R => "fun _ -> assert false".
+Extract Inlined Constant Fappli_IEEE.round_mode => "fun _ -> assert false".
+Extract Inlined Constant Fcalc_bracket.inbetween_loc => "fun _ -> assert false".
+(* Go! *)
+
+Cd "sep_extraction".
+
+Separate Extraction main print_Z svToStr posToStateVar'.
+
+Cd "..".
