formal/diguty/debug_printers.v
@@ -1,0 +1,12 @@
+(* Functions to print common data types. *)
+Require Import DigUty.float_text_io.
+
+Import FloatIO.
+
+Module DebugIO.
+Definition width := 14%nat.
+Definition fdigs := 9%nat.
+Definition print_float := float_to_string width fdigs.
+Definition print_Z := Z_to_string_base10 1%nat.
+
+End DebugIO.
