formal/diguty/extract.v
@@ -1,0 +1,32 @@
+Require Import DigUty.float_text_io.
+Import FloatIO.
+Require Import DigUty.debug_printers.
+Import DebugIO.
+
+(* Standard lib *)
+Require Import ExtrOcamlBasic.
+Require Import ExtrOcamlString.
+
+(* Coqlib *)
+Extract Inlined Constant Coqlib.proj_sumbool => "(fun x -> x)".
+
+(* Datatypes *)
+Extract Inlined Constant Datatypes.fst => "fst".
+Extract Inlined Constant Datatypes.snd => "snd".
+
+(* Avoid name clashes *)
+Extraction Blacklist List String Int.
+
+(* Cutting the dependency to R. *)
+Extract Inlined Constant Fcore_defs.F2R => "fun _ -> assert false".
+Extract Inlined Constant Fappli_IEEE.FF2R => "fun _ -> assert false".
+Extract Inlined Constant Fappli_IEEE.B2R => "fun _ -> assert false".
+Extract Inlined Constant Fappli_IEEE.round_mode => "fun _ -> assert false".
+Extract Inlined Constant Fcalc_bracket.inbetween_loc => "fun _ -> assert false".
+(* Go! *)
+
+Cd "extraction".
+Separate Extraction Z_to_float nat_power_of_float Z_to_string_base10 pad_to_width float_to_string
+           strToFloat strToFloat' print_float print_Z.
+
+Cd "..".
